progress on 16

scrap.v
@@ -1,1110 +1,2093 @@
 Set Warnings "-notation-overridden,-parsing".
 From Coq Require Import Bool.Bool Init.Nat Arith.Arith Arith.EqNat
-     Init.Datatypes Strings.String Program Sumbool.
+     Init.Datatypes Strings.String Program Logic.FunctionalExtensionality.
 Require Export Coq.Strings.String.
-From mathcomp Require Import ssrnat ssreflect ssrfun ssrbool eqtype fintype seq.
-From extructures Require Import ord fset fmap.
-Implicit Types m: {fmap nat -> nat}.
+From mathcomp Require Import ssreflect ssrfun ssrbool eqtype seq fintype ssrnat ssrfun.
+From TLC Require Import LibTactics LibLogic.
+From Semantics Require Export programs semantics algorithms lemmas_1
+lemmas_0. (*shouldn't have to import both of these*)
 
+Implicit Types N: nvmem.
 
-Definition sub_map m1 m2 := 
-  {in domm m1, m1 =1 m2}.
-
-Lemma update_sub {m1 m2}: sub_map m1 m2 ->
-                            (unionm m1 m2) = m2.
-  move => Hsub. Check eq_fmap.
-  apply/eq_fmap => x. rewrite unionmE.
-  case E: (m1 x) => [a | ] //=.
-  rewrite/sub_map in Hsub.
-  by have /Hsub <- : x \in (domm m1) by rewrite mem_domm E.
-  Qed.
-
-
-
-  (*/= := simpl
-   // := try done
-   //= := simpl; done
-{} works for any universal quantifier
-   *)
-
-
-(*basic seq functions that I couldn't find in a library*)
-Fixpoint eq_seqs {A: Type} (L1: seq A) (L2: seq A) (eq: A -> A -> Prop) :=
-        match L1, L2 with
-          nil, nil => True
-        | (w::ws), (d::ds) => (eq w d) /\ (eq_seqs ws ds eq) (*considers order*)
-        | _ , _ => False end.
-
-Fixpoint member {A: Type} (eq: A -> A -> bool) (a: A)  (L: seq A) :=
-  match L with
-    [::] => false
-  | x::xs => orb (eq a x) (member eq a xs)
-  end.
-
-Definition prefix {A: Type} (O1: seq A) (O2: seq A) :=
-  exists(l: nat), O1 = take l O2.
-
-Definition intersect {A: eqType} (O1: seq A) (O2: seq A) :=
-  exists(l: A), l \in O1 /\ l \in O2.
-
-
-Definition bar := forall n: nat, n= 0.
-Definition foo := fun n: nat => n = 0.
-
-
-Fixpoint loop (n: nat) : unit := let _ := (loop n) in tt.
-
-Compute (loop 0).
-
-(*Eval cbv in (loop 0).*)
-
-Print loop.
-
-(*Goal forall n : nat, (fix loop (n: nat) := n) n = n.
-  intros n.
-  destruct n.
-  reflexivity. Qed.*)
-
-(*Goal forall n : nat, (fun x=> x) n = n.
-  reflexivity.
-
-Goal (fun x => x) 42 = 42.
-  reflexivity.
-
-Goal bar = forall n: nat, foo n.
-  reflexivity.
-  unfold foo. reflexivity.*)
-
-
-
-Open Scope string_scope.
-(*---*)
-
-
-(*setting up strings equality type*)
-(* eqb_string and
-eqb_string_true_iff taken from software foundations*)
-Definition eqb_string (x y : string) : bool :=
-  if string_dec x y then true else false.
-
-Lemma eqb_string_true_iff : forall x y : string,
-    eqb_string x y = true <-> x = y.
-Proof.
-   intros x y.
-   unfold eqb_string.
-   destruct (string_dec x y) as [H |Hs].
-   - subst. split. reflexivity. reflexivity.
-   - split.
-     + intros contra. discriminate contra.
-     + intros H. rewrite H in Hs *. destruct Hs. reflexivity.
-Qed.
-(*what is the star*)
-Lemma eqstring: Equality.axiom eqb_string.
-Proof.
-  unfold Equality.axiom. intros.
-  destruct (eqb_string x y) eqn:beq.
-  - constructor. apply eqb_string_true_iff in beq. assumption.
-  -  constructor. intros contra. apply eqb_string_true_iff in contra.
-     rewrite contra in beq. discriminate beq.
-Qed.
-Canonical string_eqMixin := EqMixin eqstring.
-Canonical string_eqtype := Eval hnf in EqType string string_eqMixin.
-(***)
-
-
-(*Now, to business! Below is syntax*)
 Open Scope type_scope.
 
-Inductive boptype :=
-  Plus
-| Sub
-| Mult
-| Div
-| Mod
-| Or
-| And.
 
-(*shortcut!*)
-Inductive value :=
-    Nat (n: nat)
-  | Bool (b: bool)
-  | error. 
-Coercion Bool : bool >-> value.
-Coercion Nat : nat >-> value.
-
-Definition eqb_value (x y: value) :=
-  match x, y with
-    Nat nx, Nat ny => nx == ny
-  | Bool bx, Bool byy => bx == byy
-  | error, error => true
-  | _, _ => false
-  end.
-
-Lemma eqb_value_true_iff : forall x y : value,
-    is_true(eqb_value x y) <-> x = y.
-Proof.
-  intros. destruct x, y; split; simpl; 
-            try (move/eqP ->); try (intros H; inversion H); auto.
-Qed.
-
-(*look in here!*)
-(*Lemma eqb_value_true_iff1 : forall x y : value,
-    is_true(eqb_value x y) <-> x = y.
-Proof.
-  intros. destruct x, y; split; simpl; try (intros H; discriminate H).
-  - move/eqP ->. reflexivity.
-  - by move => [->].
-  - move/eqP ->. reflexivity.
-  - intros H. inversion H. apply eq_refl.
-  - auto.
-  - auto.*)
-
-    (*move => []*)
-
-Lemma eqvalue: Equality.axiom eqb_value.
-Proof.
-  unfold Equality.axiom. intros.
-  destruct (eqb_value x y) eqn:beq.
-  - constructor. apply eqb_value_true_iff in beq. assumption.
-  -  constructor. intros contra. apply eqb_value_true_iff in contra.
-     rewrite contra in beq. discriminate beq.
-Qed.
-Canonical value_eqMixin := EqMixin eqvalue.
-Canonical value_eqtype := Eval hnf in EqType value value_eqMixin.
-
-(*evaluation rules for binary operations*)
-
-Fixpoint bopeval (bop: boptype) (v1 v2 :value): (value) :=
-  match bop with
-   Plus => 
-    (
-      match v1, v2 with
-        (Nat n1), (Nat n2) => Nat (add n1 n2)
-        | _, _ => error
-        end
-    )
-  | Sub => 
-    (
-      match v1, v2 with
-       (Nat n1), (Nat n2) => Nat (n1 - n2)
-        | _, _ => error
-        end
-    )
-  | Mult => 
-    (
-      match v1, v2 with
-       (Nat n1), (Nat n2) => Nat (mul n1 n2)
-        | _, _ => error
-        end
-    )
-  | Div =>
-    (
-      match v1, v2 with
-       (Nat n1), (Nat n2) =>
-                    ( if (n2 == 0) then error
-                      else Nat (n1 / n2))
-        | _, _ => error
-        end
-    )
-  | Mod =>
-    (
-      match v1, v2 with
-       (Nat n1), (Nat n2) =>
-                    ( if (n2 == 0) then error
-                     else Nat (n1 mod n2))
-        | _, _ => error
-        end
-    )
-  | Or =>
-  (
-      match v1, v2 with
-        (Bool b1), (Bool b2) => Bool (orb b1 b2)
-        | _, _ => error
-        end
-    )
-  | And =>
-  (
-      match v1, v2 with
-        (Bool b1), (Bool b2) => Bool (andb b1 b2)
-        | _, _ => error
-        end
-  )
-  end.
-
-(*value helper functions*)
-Definition isvaluable (v: value) :=
-  match v with
-    error => False
-  | _ => True
-  end.
-
-Definition isvalidbop (bop: boptype) (v1 v2 : value) :=
-  match (bopeval bop v1 v2) with
-    error => False
-  | _ => True
-  end.
-
-
-(*memory maps...used for both memories and checkpoints*)
-Definition map_t (A: eqType) := A -> value.
-
-(*memory helpers*)
-Definition emptymap A :(map_t A) := (fun _ => error).
-Definition updatemap {A} (m: map_t A) (i: A) (v: value) : map_t A := (fun j =>
-                                                               if (j ==i) then v
-                                                               else (m j)).
-Notation "i '|->' v ';' m" := (updatemap m i v)
-  (at level 100, v at next level, right associativity).
-(*in (m1 U! m2), m1 is checked first, then m2*)
-
-Definition indomain {A} (m: map_t A) (x: A) :=
-  match m x with
-    error => False
-  | _ => True
-  end.
-(*this function is NOT used to check the domain of checkpoint maps.
- In particular, because an entire array can be checkpointed even if only
- one element has been assigned to (while the other elements may, in theory, still be unassigned),
-(in particular, I refer to D-WAR-CP-Arr)
-this function would return that assigned array elements are in the domain of N, while the unassigned array
-elements are not, even though both have been checkpointed.
- I resolved this problem by defining indomain_nvm, used for checkpoint maps in algorithms.v, which
-checks if a warvar is in the domain, rather than checking a location.
- *)
-(******************************************************************************************)
-
-(*******************************more syntax**********************************************)
-Inductive array :=
-  Array (s: string) (l: nat).
-
-Definition get_length (a: array) :=
-  match a with
-    Array _ length => length end.
-
-Inductive volatility :=
-  nonvol
- | vol.
-
-Inductive smallvar :=
-  SV (s: string) (q: volatility).
-
-Inductive el_loc :=
-  El (a: array) (i: ('I_(get_length a))).
-
-
-Definition equal_index (e: el_loc) (a2: array) (v: value) :=
-  match e with
-    El a1 i =>
-  match v with
-    Nat j => ((nat_of_ord i) = j) /\ (a1 = a2)
-  | _ => False end
-  end.
-
-
-(*'I_5 the type of all naturals < 5*)
-
-Check (enum _).
-
-Check enum [pred x: 'I_5 | true].
-
-Check enum 'I_5.
-
-
-(*want:
- do I even have to work with the nats?*)
-
-Compute enum [pred x : 'I_5 | true].
-
-Check [pred x: 'I_5 | x < 3 ].
-
-Check simpl_pred.
-
-Check 'I_4.
-
-Definition test (n: nat) :=
-  'I_n.
-
-
-
-(*used subtypes to enforce the fact that only some expressions are
- memory locations
-Definition elpred  := (fun x=> match x with
-                                        El (Array _ length) (Nat i) => (i <? length)
-                            | _ => false                                            
-                            end).
-(*elpred checks if index is a natural in bounds*)
-
-Notation el_old := {x: el_loc | elpred x}.
-
-Check SubType el.*)
-
-Inductive exp :=
-  Var (x: smallvar) 
-| Val (v: value)
-| Bop (bop: boptype) (e1: exp) (e2: exp) 
-| El_loc (e: el_loc)
-| Element (a: array) (e: exp). (*good that you let in out of bounds arrays here because it means that
-                           war bugs of that kind can still get in at the type level,
-                           need the CP system*)
-Coercion Val : value >-> exp.
-Coercion Var : smallvar >-> exp.
-Notation "a '[[' e ']]'" := (Element (a) (e))
-                              (at level 40, right associativity).
-
-Coercion El_loc : el_loc >-> exp.
-
-Definition loc := smallvar + el_loc. (*memory location type*)
-
-Definition index_loc (a: array) (i: ('I_(get_length a))) : loc :=
-  inr (El a i).
-
-Definition generate_locs (a: array): seq loc :=
-  map (index_loc a) (enum ('I_(get_length a))).
-Notation warvars := (seq loc).
-(*Coercion (inl smallvar el): smallvar >-> loc.*)
-(*Coercion inl: smallvar >-> loc.*)
-
-(**location and warvar helper functions*)
-(**no need to work directly with the subtypes or sumtypes, just use these**)
-(**Note: some of these are currently unused due to implementation changes, but I left them
- as they might be useful later*)
-
-(*array and el functions*)
-
-(*equality type for arrays*)
-Open Scope seq_scope.
-Definition eqb_array (a1 a2: array) :=
-  match a1, a2 with
-    Array s1 l1, Array s2 l2 => andb (s1 == s2) (l1 == l2)
-  end.
-
-Lemma eqb_array_true_iff : forall x y : array,
-    is_true(eqb_array x y) <-> x = y.
-Proof.
-  intros. destruct x, y; split; simpl.
-  - move/(reflect_conj eqP eqP).
-    case => H0 H1. subst. reflexivity.
-  - intros H. inversion H.
-    apply (introT (reflect_conj eqP eqP)). (*ask arthur is there a
-                                            way to do this using ssreflect
-                                            rather than the introT
-                                            lemma*)
-    split; reflexivity.
-Qed.
-
-Lemma eqarray: Equality.axiom eqb_array.
-Proof.
-  unfold Equality.axiom. intros.
-  destruct (eqb_array x y) eqn:beq.
-  - constructor. apply eqb_array_true_iff in beq. assumption.
-  -  constructor. intros contra. apply eqb_array_true_iff in contra.
-     rewrite contra in beq. discriminate beq.
-Qed.
-Canonical array_eqMixin := EqMixin eqarray.
-Canonical array_eqtype := Eval hnf in EqType array array_eqMixin.
-(*****)
-
-(*equality type for elements*)
-
-
-Check cast_ord.
-
-
-
-Definition eqb_el_d (x y:el_loc) :=
-  match x, y with
-    El ax ix, El ay iy => (ax==ay) && ((nat_of_ord ix) == (nat_of_ord iy)) end.
-
-(*if I remove annoying does subst in the proof below behave differently?*)
-
-Lemma annoying: forall(a1 a2: array),
-    a1 == a2 -> 'I_(get_length a1) = 'I_(get_length a2).
-by move => a1 a2 / eqP ->. Qed.
-
-
-Set Printing All.
-(*tidy this up*)
-Lemma eqb_eld_iff : forall x y : el_loc,
-    is_true(eqb_el_d x y) <-> x = y.
-Proof.
-  case => [ax ix] [ay iy]. simpl.
-  split.   case / (reflect_conj eqP eqP) => [H1 H2]. subst.
-  cut (ix = iy).
-  intros. by subst.
-    by apply val_inj.
- Unset Printing All.
- move => [H1 H2].
- apply andb_true_iff. split.
-   by move / eqP : H1.
-  inversion H2. (*why does this inversion cause a loop?*)
-  by apply (introT eqP).
+(*lemmas for the lemmas; not in paper*)
+Lemma sub_disclude N0 N1 N2:  forall(l: loc),
+                     subset_nvm N0 N1 ->
+                     subset_nvm N0 N2 ->
+                     not ((getmap N1) l = (getmap N2) l)
+                     -> not (l \in (getdomain N0)).
+Proof. intros. intros contra. unfold subset_nvm in H. destruct H.
+       remember contra as contra1. clear Heqcontra1.
+       apply H2 in contra.
+       unfold subset_nvm in H0. destruct H0. apply H3 in contra1.
+       symmetry in contra.
+       apply (eq_trans _ _ _ contra) in contra1.
+       apply H1. assumption.
 Qed.
 
 
+Lemma wt_subst_fstwt: forall{C1 C2: context} {O: obseq} {W: the_write_stuff},
+      (* pose proof (cceval_to_rd_sv H H5). *)
+  trace_c C1 C2 O W ->
+    subseq (getfstwt W) (getwt W).
+Proof. intros C1 C2 O W T. induction T.
+       + auto.
+       + induction H; auto; try (unfold getfstwt; unfold getwt;
+         apply filter_subseq).
+       - simpl. apply (cat_subseq (subseq_trans
+                                    (filter_subseq _ _ )
+                                    IHT2) IHT1
+                                    ).
+Qed.
 
 
-Lemma eq_eld_iff: Equality.axiom eqb_el_d.
+Lemma trace_stops: forall {N N': nvmem} {V V': vmem}
+                    {l: instruction} {c: command}
+  {O: obseq} {W: the_write_stuff},
+    trace_c (N, V, Ins l) (N', V', c) O W ->
+    (c = Ins l) \/ (c = skip).
 Proof.
-  unfold Equality.axiom. intros.
-  destruct (eqb_el_d x y) eqn:beq.
-  - constructor. apply eqb_eld_iff in beq. assumption.
-  -  constructor. intros contra. apply eqb_eld_iff in contra.
-     rewrite contra in beq. discriminate beq.
-Qed.
-Check SubEqMixin.
-Check EqMixin.
-Check Equality.mixin_of.
-Canonical eld_eqMixin := EqMixin eq_eld_iff.
-Canonical eld_eqtype := Eval hnf in EqType el_loc eld_eqMixin.
-(*suggests it wants an equality relation for the big type before it lets
- you have it for the subtype...that's annoying...ask arthur*)
-
-
-(*smallvar functions*)
-Definition isNV_b (x: smallvar) := (*checks if x is stored in nonvolatile memory*)
-  match x with
-    SV _ nonvol => true
-  | _ => false
-  end.
-
-Definition isV_b (x: smallvar) :=(*checks if x is stored in volatile memory*)
-  match x with
-    SV _ vol => true
-  | _ => false
-  end.
-
-Definition isNV x := is_true(isNV_b x). (*prop version of isNV_b*)
-
-Definition isV x := is_true(isV_b x). (*prop version of isV_b*)
-
-Definition eqb_smallvar (x y: smallvar): bool :=
-  match x, y with
-    SV sx vol, SV sy vol => sx== sy
-  | SV sx nonvol, SV sy nonvol => sx== sy
-  | _, _ => false end.                                     
-
-Lemma eqb_smallvar_iff : forall x y : smallvar,
-    is_true(eqb_smallvar x y) <-> x = y.
-Proof.
-  intros. destruct x, y, q, q0; simpl;
-     try (split; [move/ eqP ->; reflexivity |
-                  intros H; inversion H; auto]);
-  try (split; [case => H; discriminate H | case => H H1; inversion H1]).
+  intros N N' V V' l c O W T. dependent induction T.
+  + constructor.
+  + reflexivity.
+  + inversion H; subst; try(right; reflexivity).
+  + destruct3 Cmid nmid vmid cmid.
+    assert (cmid = l \/ cmid = skip).
+    {
+      apply (IHT1 N nmid V vmid l cmid); reflexivity.
+    }
+  + inversion H1; subst.
+       -  eapply IHT2; reflexivity.
+       - right.
+         destruct (IHT2 nmid N' vmid V' skip c); (reflexivity || assumption).
 Qed.
 
-Lemma eqsmallvar: Equality.axiom eqb_smallvar.
-Proof.
-  unfold Equality.axiom. intros.
-  destruct (eqb_smallvar x y) eqn:beq.
-  - constructor. apply eqb_smallvar_iff in beq. assumption.
-  -  constructor. intros contra. apply eqb_smallvar_iff in contra.
-     rewrite contra in beq. discriminate beq.
+Lemma observe_checkpt: forall {N N': nvmem} {V V': vmem}
+                     {c c': command} {w: warvars}
+                    {O: obseq} {W: the_write_stuff},
+    trace_c (N, V, (incheckpoint w ;; c)) (N', V', c') O W ->
+    c' = (incheckpoint w ;; c) \/ checkpoint \in O.
+  intros N N' V V' c c' w O W T.
+  dependent induction T.
+  + left. reflexivity.
+  +  inversion H; subst. right.  apply(mem_head checkpoint).
+     inversion H11.
+  + destruct3 Cmid nmid vmid cmid. destruct (IHT1 N nmid V vmid c cmid w); subst; try reflexivity.
+      - destruct (IHT2 nmid N' vmid V' c c' w); subst; try reflexivity;
+          [left; reflexivity | right; apply (in_app_r H1)].
+      - right. apply (in_app_l H1).
 Qed.
 
-Canonical smallvar_eqMixin := EqMixin eqsmallvar.
-Canonical smallvar_eqtype := Eval hnf in EqType smallvar smallvar_eqMixin.
-
-(*loc and warvar functions*)
-
-Definition eqb_loc (l1: loc) (l2: loc) :=
-  match l1, l2 with
-    inl x, inl y => x == y
-  | inr x, inr y => x == y
-  | _, _ => false 
-  end.
-
-(*equality type for locations*)
-
-Lemma eqb_loc_true_iff : forall x y : loc,
-    is_true(eqb_loc x y) <-> x = y.
-Proof.
-  case => [x1 | x2] [y1 | y2]; simpl; split; try (by move/ eqP ->);
-      try (by move => [] ->); intros H; inversion H.
-Qed.
-
-Lemma eqloc: Equality.axiom eqb_loc.
-Proof.
-  unfold Equality.axiom. intros.
-  destruct (eqb_loc x y) eqn:beq.
-  - constructor. apply eqb_loc_true_iff in beq. assumption.
-  -  constructor. intros contra. apply eqb_loc_true_iff in contra.
-     rewrite contra in beq. discriminate beq.
-Qed.
-Canonical loc_eqMixin := EqMixin eqloc.
-Canonical loc_eqtype := Eval hnf in EqType loc loc_eqMixin.
-
-
-
-(*******************************************************************)
-
-(*more syntax*)
-Inductive instruction :=
-  skip
-| asgn_sv (x: smallvar) (e: exp) (*could distinguish between NV and V assignments as well here*)
-| asgn_arr (a: array) (i: exp) (e: exp) (*i is index, e is new value of a[i]*)
-| incheckpoint (w: warvars)
-| inreboot.
-(*added the in prefixes to distinguish from the observation reboots
- and checkpoints*)
-
-Inductive command :=
-  Ins (l: instruction)
-| Seqcom (l: instruction) (c: command) (*added suffix to distinguish from Seq ceval
-                                         constructor*)
-| ITE (e: exp) (c1: command) (c2: command).
-
-Notation "l ';;' c" := (Seqcom l c)
-  (at level 41, right associativity).
-
-Notation "'TEST' e 'THEN' c1 'ELSE' c2 " := (ITE e c1 c2)
-                                              (at level 100).
-Coercion Ins : instruction >-> command.
-
-(*******************************************************************)
-
-(******setting up location equality relation for memory maps******************)
-(****************************************************************)
-
-(****************************memory*************************************)
-
-(*memory locations defined above warvars*)
-Notation mem := (map_t loc_eqtype). (*memory mapping*)
-
-Inductive nvmem := (*nonvolatile memory*)
-  NonVol (m : mem) (D: warvars). (*extra argument to keep track of checkpointed warvars because
-                                  it might be nice to have for when we do checkpoint proofs*)
-
-Inductive vmem := (*volatile memory*)
-  Vol (m : mem).
-
-(*I could change nvmem and vmem to enforce that they only take in smallvars
- of the correct type but it's already checked in my evaluation rules*)
-
-(**************************helpers for the memory maps*********************************************)
-
-(*note: a lot of these aren't being used right now because, after I changed the types
- of DINO and WAR, they aren't necessary.
- I won't delete them because having the domain of the checkpoint easily accessible and
- manipulable could be handy in the future*)
-
-Definition getmap (N: nvmem) :=
-  match N with NonVol m _ => m end.
-
-Definition getdomain (N: nvmem) :=
-  match N with NonVol _ D => D end.
-
-Definition getvalue (N: nvmem) (i: loc) :=
-  (getmap N) i.
-  Notation "v '<-' N" := (getvalue N v)
-                           (at level 40).
-
-
-  (*updates domain and mapping function*)
-  (*start here consider defining the two below in terms of updatemaps
-   for more generality in proofs
-   actually dont do this cuz domain weirdness in updatemaps makes it so that
-   you'd have a nested if in update_arr which you'll need to use
-   in all the eval proofs*)
-Definition updateNV_sv (N: nvmem) (i: smallvar) (v: value) :=
-  match N with NonVol m D =>
-               NonVol (updatemap m (inl i) v) ((inl i):: D)  end.
-
-
-(*this one should only be called within in eval*)
-(*adds ENTIRE array to domain for checkpoint utility*)
-Definition updateNV_arr (N: nvmem) (i: el_loc) (a: array) (v: value) :=
-  match N with NonVol m D =>
-               NonVol (updatemap m (inr i) v) ((generate_locs a) ++ D)  end.
-
-(*used to update NV memory with checkpoint*)
-(*checks N first, then N'*)
-Definition updatemaps (N: nvmem) (N': nvmem): nvmem :=
-  match N, N' with
-    NonVol m D, NonVol m' D' => NonVol
-   (fun j =>
-      if (j \in D)
-          then (m j)
-          else (m' j))
-  (D ++ D') (*inclusion of duplicates*)
-  end.
-Notation "m1 'U!' m2" := (updatemaps m1 m2) (at level 100).
-(*start here should really change the above ordering to be more intuitive*)
-
-Notation emptyNV := (NonVol (emptymap loc_eqtype) nil).
-Definition reset (V: vmem) := Vol (emptymap loc_eqtype).
-
-(*restricts memory map m to domain w*)
-(*doesn't actually clean the unnecessary variables out of m*)
-(*need a decidable In here*)
-Lemma decidable_loc: forall(x y: loc), {x = y} + {x <> y}.
-  intros. destruct (x == y) eqn: beq.
-  apply left. apply: eqP beq.
-  apply right. apply (elimF eqP beq).
-Qed.
-(*start here how to use the reflect/move stuff when things
- are false*)
-
-(*Lemma decidable_in: forall(x: loc) (w: warvars),
-    {In x w} + {not (In x w)}.
-apply (in_dec decidable_loc). Qed.*)
-
-
-(*removes L1 from L2 *)
-Definition remove (L1 L2 : seq loc) :=
-  filter (fun x =>  negb (x \in L1)) L2.
-
-Definition restrict (N: nvmem) (w: warvars): nvmem :=
-  match N with NonVol m D => NonVol
-    (fun input => if (input \in w) then m input else error) w  end.
-
-Notation "N '|!' w" := (restrict N w) 
-  (at level 40, left associativity).
-
-(*prop determining if every location in array a is in the domain of m*)
-Definition indomain_nvm (N: nvmem) (w: loc) :=
-  w \in (getdomain N).
-
-(*equality type for seq loc
-
-Fixpoint eqb_warvars (w1: warvars) (w2: warvars) :=
-  match w1, w2 with
-    [::], [::] => true
-  | (x::xs), (y::ys) => (x == y) && (eqb_warvars xs ys)
-  | _, _ => false 
-  end.
-
-Lemma eqb_wv_refl: forall y: warvars, is_true (eqb_warvars y y).
+Lemma observe_rb:forall {C0 C1: context} {N N': nvmem} {V V': vmem}
+                     {c': command} 
+                    {O: obseq} {W: the_write_stuff},
+    trace_i (C0, N, V, (Ins inreboot)) (C1, N', V', c') O W ->
+    c' = (Ins inreboot) \/ reboot \in O.
   Admitted.
 
-Lemma eqb_wv_true_iff : forall x y : warvars,
-    is_true(eqb_warvars x y) <-> x = y.
-Proof.
-  intros. induction x.
-  + split. destruct y. simpl. auto.
-    unfold eqb_warvars. simpl. intros contra. discriminate contra.
-    move ->. Admitted.
-
-Lemma eqwv: Equality.axiom eqb_warvars.
-Proof.
+(*consider another type where reboot is the principle break
+ between continuous and intermittent
+ and then you wouldnt need this guy*)
+Lemma neg_observe_rb: forall {N N': nvmem} {V V': vmem}
+                     {c c': command} 
+                    {O: obseq} {W: the_write_stuff},
+    trace_c (N, V, c) (N', V', c') O W ->
+    reboot \notin O.
 Admitted.
 
-Canonical wv_eqMixin := EqMixin eqwv.
-Canonical wv_eqtype := Eval hnf in EqType warvars wv_eqMixin.*)
 
-Definition test1 :warvars := [::inl( SV "h" nonvol)].
-Definition test2 :warvars := [::inl(SV "f" nonvol)].
-Compute test1 == test2.
-
-
-Definition isdomain_nvm (N: nvmem) (w: warvars) :=
-  (getdomain N) == w.
-Definition subset_nvm (N1 N2: nvmem) :=
-  (subseq (getdomain N1) (getdomain N2)) /\ (forall(l: loc),
-                                    l \in (getdomain N1) ->
-                                    (getmap N1) l = (getmap N2) l
-                                  ).
-(********************************************)
-Inductive cconf := (*continuous configuration*)
-  ContinuousConf (triple: nvmem * vmem * command).
-
-Notation context := (nvmem * vmem * command).
-
-(*A coercion for cconf doesn't work because it's the same essential type as context.
- So, in practice, to avoid writing the constructor everywhere, I've been using contexts foralleverything, when conceptually a cconf would make more sense.
- It would be nice to just have one type for this.*)
-
-Notation iconf := (context * nvmem * vmem * command).
-
-Definition getcom (C: context) :=
-  match C with
-    (_, _, out) => out end.
-
-Definition ro := loc * value. (*read observation*)
-Definition readobs := seq ro.
-
-Notation NoObs := (nil : readobs).
-
-Inductive obs := (*observation*)
-  Obs (r: readobs)
-| reboot
-| checkpoint.
-Coercion Obs : readobs >-> obs.
-
-(*equality type for obs*)
-Definition eqb_ro (ro1: ro) (ro2: ro) :=
-  match ro1, ro2 with
-    (l1, v1), (l2, v2) => (l1 == l2) && (v1 == v2)
-  end.
-
-Lemma eqb_ro_true_iff : forall x y : ro,
-    is_true(eqb_ro x y) <-> x = y.
-Proof.
-  case => [l1 v1] [l2 v2]. split.
-  simpl. case / andP. by repeat move / eqP ->.
-  case. repeat move ->. unfold eqb_ro.
-apply / andP. by split. 
+Lemma negNVandV: forall(x : smallvar), isNV x -> not (isV x).
+Proof. unfold isNV. unfold isV.
+       unfold isNV_b. unfold isV_b.
+       move => [s v]. destruct v; auto. (*ask arthur do both destructs at once?*)
 Qed.
 
-Lemma eqro: Equality.axiom eqb_ro.
-Proof.
-  unfold Equality.axiom. intros.
-  destruct (eqb_ro x y) eqn:beq.
-  - constructor. apply eqb_ro_true_iff in beq. assumption.
-  -  constructor. intros contra. apply eqb_ro_true_iff in contra.
-     rewrite contra in beq. discriminate beq.
-Qed.
-Canonical ro_eqMixin := EqMixin eqro.
-Canonical ro_eqtype := Eval hnf in EqType ro ro_eqMixin.
+(*ask arthur difference between val and sval
+ i think it's to do with one being an equality type
+ and the other not?*)
+Set Printing Coercions.
 
-Definition eqb_obs (o1: obs) (o2: obs) :=
-  match o1, o2 with
-    reboot, reboot => true
-  | checkpoint, checkpoint => true
-  | Obs R1, Obs R2 => R1 == R2
-  | _, _ => false end.
-
-Lemma eqb_obs_true_iff : forall x y : obs,
-    is_true(eqb_obs x y) <-> x = y.
-Proof.
-  case => [ R1 | |] [R2 | | ]; split; simpl; try (intros H; discriminate H);
-  try auto.
-  + by move/ eqP ->.
-  + move => [H]. by rewrite H.
+Lemma equal_index_works: forall{e0 e1: el_loc} {a: array} {v: value},
+    equal_index e0 a v -> equal_index e1 a v ->
+    e0 = e1.
+        intros. unfold equal_index in H.
+        destruct e0.
+        destruct e1.
+        destruct v eqn: veq; try (exfalso; assumption).
+        unfold equal_index in H0.
+        destruct H, H0.
+        subst.
+        cut (i = i0).
+        intros. by subst.
+          by apply ord_inj.
 Qed.
 
-Lemma eqobs: Equality.axiom eqb_obs.
-Proof.
-  unfold Equality.axiom. intros.
-  destruct (eqb_obs x y) eqn:beq.
-  - constructor. apply eqb_obs_true_iff in beq. assumption.
-  -  constructor. intros contra. apply eqb_obs_true_iff in contra.
-     rewrite contra in beq. discriminate beq.
+Lemma equal_index_arr: forall{a0 a: array} {i: 'I_(get_length a0)}
+                           {v: value},
+    equal_index (El a0 i) a v -> a0 = a.
+        intros. unfold equal_index in H.
+        destruct v eqn: veq; try (exfalso; assumption).
+        destruct H. assumption.
 Qed.
-Canonical obs_eqMixin := EqMixin eqobs.
-Canonical obs_eqtype := Eval hnf in EqType obs obs_eqMixin.
 
-Notation obseq := (seq obs). (*observation sequence*)
+Lemma gen_locs_works: forall{a a0: array} {i: 'I_(get_length a0)}
+                           {v: value},
+    equal_index (El a0 i) a v -> (inr (El a0 i)) \in (generate_locs a).
+  intros. apply equal_index_arr in H. subst.
+  unfold generate_locs. unfold index_loc.
+  destruct a.
+  simpl in i.
+  simpl.  intros.
+  Check inE.
+  apply (map_f (fun i0 => inr (El (Array s l) i0)))
+  .
+  by rewrite mem_enum.
+Qed.
+  (*suffices: 
+  rewrite <- inE.
+  induction i.
+    intros H.
+  destruct a. simpl.
+  simpl in H.
+  injection.
+  unfold enum in H.
+  unfold in_mem.
+  unfold in_mem in H.
+  unfold pred_of_mem.
+  unfold mem_seq_predType.
+  apply H.
+
+  unfold equal_index in H.
+        destruct v eqn: veq; try (exfalso; assumption).
+        destruct H. assumption.
+Qed.*)
+
+(*consider using map cat for the app thing*)
+Lemma determinism_e: forall{N: nvmem} {V: vmem} {e: exp} {r1 r2: readobs} {v1 v2: value},
+    eeval N V e r1 v1 ->
+    eeval N V e r2 v2 ->
+    r1 = r2 /\ v1 = v2.
+Proof. intros N V e r1 r2 v1 v2 H. move: r2 v2. (*ask arthur; does GD not do what
+                                                      I want here bc it's a prop?*)
+       dependent induction H.
+       + intros r2 v2 H2. dependent induction H2. split; reflexivity.
+       + intros r0 v0 H2.
+         dependent induction H2.
+         appldis IHeeval1 H2_.
+         appldis IHeeval2 H2_0.
+         subst. split; reflexivity.
+       + intros r2 v2 H2. inversion H2; subst.
+         - split; reflexivity.
+         - exfalso. apply (negNVandV x); assumption.
+       + intros r2 v2 H2. inversion H2; subst.
+         - exfalso. apply (negNVandV x); assumption.
+         - split; reflexivity.
+       + intros r2 v2 H2nd. inversion H2nd. subst.
+         appldis IHeeval H5. subst.
+         cut (element = element0).
+        intros. subst.
+        split; reflexivity.
+        apply (equal_index_works H1 H9).
+        Qed.
+
+(*I try to use the same names in all branches for automation
+ and it tells me "name" already used!*)
+Lemma determinism_c: forall{C1 C2 C3: context} {O1 O2: obseq} {W1 W2: the_write_stuff},
+    cceval_w C1 O1 C2 W1 ->
+    cceval_w C1 O2 C3 W2 ->
+    C2 = C3 /\ O1 = O2 /\ W1 = W2.
+Proof. intros C1 C2 C3 O1 O2 W1 W2 cc1 cc2. destruct C1 as [blah c]. destruct blah as [N V].
+       destruct3 C2 N2 V2 com2. 
+       generalize dependent C3.
+       generalize dependent O2.
+       generalize dependent W2.
+ induction cc1; intros; inversion cc2 as
+           [| | | | | N20 N2' V20 V2' l20 c20 o20 W20| | ]
+       (*only put vars for 1 branch but all changed? start here do not ask
+        arthur this*)
+       ; subst; try (exfalso; eapply (negNVandV x); assumption);
+         try (destruct (determinism_e H H2); subst);
+         try (exfalso; apply (H w); reflexivity);
+         try (exfalso; (apply H1 || apply H0); reflexivity);
+         try (destruct (determinism_e H H0); inversion H2);
+         try (apply IHcc1 in H3; destruct H3 as
+             [onee rest]; destruct rest as [two threee];
+              inversion onee; inversion two);
+         try( 
+ destruct (determinism_e H3 H); destruct (determinism_e H4 H0); subst;
+   pose proof (equal_index_works H1 H5));
+         try (subst;
+              split; [reflexivity | (split; reflexivity)]).
+Qed.
 
 
-(*helpers for configs*)
-Inductive single_com: context -> Prop :=
-  SingleCom: forall(N: nvmem) (V: vmem) (l: instruction),
-               single_com (N, V, Ins l).
-
-Definition single_com_i (C: iconf) :=
-  match C with (_, _, c) =>
-  (match c with
-    Ins _ => True
-  | _ => False end) end.
-
-(*helpers for observations and warvars*)
-
-(*converts from seq of read locations to list of
-WAR variables
- *)
-
-(*Fixpoint readobs_wvs (R: readobs): (seq loc) := 
-  match R with
-    nil => nil
-  | (r::rs) => (fst r) :: (readobs_wvs rs)
-  end.*)
-
-Definition getwvs (l: loc) :=
-  match l with
-    inl x => [::l]
-  | inr (El a _) => (generate_locs a) end.
-
-Fixpoint readobs_wvs (R: readobs): (seq loc) := 
-  match R with
-    nil => nil
-  | (r::rs) => getwvs(fst r) ++ (readobs_wvs rs)
-  end.
-
-
-(*relations between continuous and intermittent observations*)
-(*Definition reduces (O1 O2: readobs) :=
-  (prefix O1 O2*)
-Notation "S <= T" := (prefix S T).
-
-(*Where
-O1 is a sequence of read observation seqs,
-where each continguous read observation seq is separated from those adjacent to it by a reboot,
-and O2 is a read observation seq,
-prefix_seq determines if each ro seq in O1 is a valid
-prefix of O2*)
-Inductive prefix_seq: obseq -> obseq -> Prop :=
-  RB_Base: forall(O: readobs), prefix_seq [:: Obs O] O
-| RB_Ind: forall(O1 O2: readobs) (O1': obseq),
-    O1 <= O2 -> prefix_seq O1' O2 -> prefix_seq ([:: Obs O1] ++ [:: reboot] ++ O1') O2.
-
-Notation "S <=m T" := (prefix_seq S T) (at level 100).
-(* Where
-O1 is a sequence of ((read observation seq sequences), where
-each continguous read observation seq is separated from those adjacent to it
-by a reboot), where each sequence is separated from those adjacent to it by a checkpoint.
-ie, each read observation seq in a given read observation sequence
-occurs within the same checkpointed region as all the other read observation seqs in that sequence,
-O2 is a read observation seq,
-prefix_frag determines if each ro seq in O1 is a prefix of some FRAGMENT of O2
-(where the fragments are separated by the positioning of the checkpoints in O1)
- *)
-Inductive prefix_fragment: obseq -> readobs -> Prop :=
-  CP_Base: forall(O1: obseq) (O2: readobs), prefix_seq O1 O2 -> prefix_fragment O1 O2
-| CP_IND: forall(O1 O1': obseq) (O2 O2': readobs),
-    prefix_seq O1 O2 -> prefix_fragment O1' O2' ->
-   prefix_fragment (O1 ++ [:: checkpoint] ++ O1') (O2 ++ O2'). 
-
-(***************************************************************)
-
-
-(****************continuous operational semantics***********************)
-(*evaluation relation for expressions*)
-
-Inductive eeval: nvmem -> vmem -> exp -> readobs -> value -> Prop :=
-  VAL: forall(N: nvmem) (V: vmem) (v: value),
-    (isvaluable v) -> (*extra premise to check if v is valuable*)
-    eeval N V v NoObs v
-| BINOP: forall(N: nvmem) (V: vmem)
-          (e1: exp) (e2: exp)
-          (r1: readobs) (r2: readobs)
-          (v1: value) (v2: value) (bop: boptype),
-    eeval N V e1 r1 v1 ->
-    eeval N V e2 r2 v2 -> 
-    (isvalidbop bop v1 v2) -> (*extra premise to check if v1, v2, bop v1 v2 valuable*)
-    eeval N V (Bop bop e1 e2) (r1++ r2) (bopeval bop v1 v2)
-| RD_VAR_NV: forall(N: nvmem) (mapV: vmem) (x: smallvar) (v: value),
-    ((inl x) <-N) = v ->
-    isNV(x) -> (*extra premise to make sure x is correct type for NV memory*)
-    (isvaluable v) -> (*extra premise to check if v is valuable*)
-    eeval N mapV x [:: ((inl x), v)] v
-| RD_VAR_V: forall(N: nvmem) (mapV: mem) (x: smallvar) (v: value),
-    (mapV (inl x)) = v ->
-    isV(x) -> (*extra premise to make sure x is correct type for V memory*)
-    (isvaluable v) -> (*extra premise to check if v is valuable*)
-    eeval N (Vol mapV) x [:: ((inl x), v)] v
-| RD_ARR: forall(N: nvmem) (V: vmem)
-           (a: array)
-           (index: exp)
-           (rindex: readobs)
-           (vindex: value)
-           (element: el_loc)
-           (v: value),
-    eeval N V (index) rindex vindex ->
-    ((inr element) <-N) = v ->
-    equal_index element a vindex -> (*extra premise to check that inr element
-                                        is actually a[vindex] *)
-(*well-typedness, valuability, inboundedness of vindex are checked in elpred*)
-    (isvaluable v) -> (*extra premise to check if v is valuable*)
-    eeval N V (a[[index]]) (rindex++[:: ((inr element), v)]) v
+(*concern: the theorem below is not true for programs with io
+ but then again neither is lemma 10*)
+Lemma single_step_all: forall{C1 Cmid C3: context} 
+                    {Obig: obseq} {Wbig: the_write_stuff},
+    trace_c C1 C3 Obig Wbig ->
+    Obig <> [::] ->
+    (exists (O1: obseq) (W1: the_write_stuff), cceval_w C1 O1 Cmid W1) ->
+    exists(Wrest: the_write_stuff) (Orest: obseq), trace_c Cmid C3 Orest Wrest
+/\ subseq Orest Obig
 .
+  intros C1 Cmid C3 Obig Wbig T OH c.
+  generalize dependent c.
+  generalize dependent Cmid.
+  remember T as Tsaved. clear HeqTsaved. (*make ltac for this*)
+  dependent induction T; intros.
+  + exfalso. apply OH. reflexivity.
+  + destruct c as [O1 rest]. destruct rest as [W1 c0]. exists emptysets (nil: obseq).
+    constructor. cut (C2 = Cmid).
+    - intros Hmid. subst. constructor. 
+    - eapply determinism_c. apply H. apply c0.
+    - apply sub0seq.
+      + assert (Tfirst: exists Wrest Orest,  (trace_c Cmid0 Cmid Orest Wrest)
+                       /\ subseq Orest O1                           
+               ) by (apply IHT1; try assumption).
+        destruct Tfirst as [Wrest rest]. destruct rest as [Orest T0mid]. destruct T0mid as [T0mid incl1].
+        exists (append_write Wrest W2) (Orest ++ O2). destruct Orest; split.
+    - simpl. apply empty_trace in T0mid. destruct T0mid.
+      subst. rewrite append_write_empty_l; auto.
+      reflexivity.
+    - simpl. apply suffix_subseq.
+    - eapply CTrace_App. apply T0mid. intros contra. inversion contra.
+      assumption. assumption.
+    - eapply cat_subseq. assumption. apply subseq_refl.
+Qed.
 
-(****************************************************************************)
+Lemma trace_steps: forall{C1 C3: context} 
+                    {Obig: obseq} {Wbig: the_write_stuff},
+    trace_c C1 C3 Obig Wbig ->
+    Obig <> [::] ->
+    exists(Csmall: context) (Osmall: obseq) (Wsmall: the_write_stuff),
+      cceval_w C1 Osmall Csmall Wsmall.
+Proof. intros C1 C3 Obig Wbig T H. induction T.
+       + exfalso. apply H. reflexivity.
+       + exists C2 O W. assumption. apply (IHT1 H0).
+Qed.
 
-(**********continuous execution semantics*************************)
-
-
-(*evaluation relation for commands*)
-
-
-
-(*written, read, written before reading*)
-Notation the_write_stuff := ((seq loc) * (list loc) * (list loc)).
-
-(*consider using a record type so I don't need so many of these*)
-
-Definition getwt (W: the_write_stuff) := match W with (out, _, _ )=> out end.
-
-Definition getrd (W: the_write_stuff) := match W with (_, out , _ )=> out end.
-
-Definition getfstwt (W: the_write_stuff) := match W with (_, _, out )=> out end.
-
-Notation emptysets := ((nil : (seq loc)), (nil: (list loc)), (nil: (list loc))).
+Lemma seq_step: forall{N: nvmem} {V: vmem} {l: instruction} {c: command}
+    {C2: context} {O: obseq} {W: the_write_stuff},
+    cceval_w (N, V, l;;c) O C2 W ->  c = (getcom C2).
+Proof.
+  intros. inversion H; subst; simpl; reflexivity.
+Qed.
 
 
-
-(***Below, I define an evaluation relation for continuous programs which accumulates
- read/write data as the program evaluates. This makes the trace type more elegant, while
- also containing the same data as the cceval above.
-However, the write data does not influence the evaluation of the program, so, if it were not
-for the trace type, it wouldn't be clear I would include this here.
-It not included in the evaluation relation in the paper.
- **)
-(*Single steps, accumulates write data*)
-(*Note: program consisting of just a checkpoint is illegal...huh*)
+Lemma if_step: forall{N: nvmem} {V: vmem} {e: exp} {c1 c2: command}
+    {C2: context} {O: obseq} {W: the_write_stuff},
+    cceval_w (N, V, (TEST e THEN c1 ELSE c2)) O C2 W ->  c1 = (getcom C2)
+\/ c2 = (getcom C2).
+  intros. inversion H; subst; simpl;( (left; reflexivity) || (right; reflexivity)).
+Qed.
 
 
-Inductive cceval_w: context -> obseq -> context -> the_write_stuff -> Prop :=
-CheckPoint: forall(N: nvmem)
-               (V: vmem)
-               (c: command)
-               (w: warvars),
-    cceval_w (N, V, ((incheckpoint w);; c))
-             (checkpoint:: nil)
-             (N, V, c)
-             (nil, nil, nil)
-| NV_Assign: forall{x: smallvar} {N: nvmem} {V: vmem} {e: exp} {r: readobs} {v: value},
-    eeval N V e r v ->
-    isNV(x) -> (*checks x is correct type for NV memory*)
-    (isvaluable v) -> (*extra premise to check if v is valuable*)
-    cceval_w (N, V, Ins (asgn_sv x e))
-             (Obs r :: nil)
-             ((updateNV_sv N x v), V, Ins skip)
-             ([:: inl x],  (readobs_wvs r), (remove (readobs_wvs r) [:: inl x]))
-| V_Assign: forall(x: smallvar) (N: nvmem) (mapV: mem) (e: exp) (r: readobs) (v: value),
-    eeval N (Vol mapV) e r v ->
-    isV(x) -> (*checks x is correct type for V memory*)
-    (isvaluable v) -> (*extra premise to check if v is valuable*)
-    cceval_w (N, (Vol mapV), Ins (asgn_sv x e)) 
-             (Obs r :: nil)
-             (N, (Vol ((inl x) |-> v ; mapV)), Ins skip)
-             (nil,  (readobs_wvs r), nil)
-| Assign_Arr: forall (N: nvmem) (V: vmem)
-               (a: array)
-               (ei: exp)
-               (ri: readobs)
-               (vi: value)
-               (e: exp)
-               (r: readobs)
-               (v: value)
-               (element: el_loc),
-    eeval N V ei ri vi ->
-    eeval N V e r v ->
-    equal_index element a vi -> (*extra premise to check that inr element
-                                        is actually a[vindex] *)
-(*well-typedness, valuability, inboundedness of vindex are checked in elpred*)
-    (isvaluable v) -> (*extra premise to check if v is valuable*)
-    cceval_w (N, V, Ins (asgn_arr a ei e))
-           ((Obs (cat ri r)) :: nil)
-           ((updateNV_arr N element a v), V, Ins skip)
-           ((generate_locs a), (readobs_wvs (cat r ri)), (remove (readobs_wvs (cat r ri)) (generate_locs a)))
-(*valuability and inboundedness of vindex are checked in sameindex*)
-| Skip: forall(N: nvmem)
-         (V: vmem)
-         (c: command),
-    cceval_w (N, V, (skip;;c)) ((Obs NoObs)::nil) (N, V, c) (nil, nil, nil)
-| Seq: forall (N N': nvmem)
-         (V V': vmem)
-         (l: instruction)
-         (c: command)
-         (o: obs)
-         (W: the_write_stuff),
-    (forall(w: warvars), l <> (incheckpoint w)) ->
-    l <> skip ->
-    cceval_w (N, V, Ins l) (o::nil) (N', V', Ins skip) W ->
-    cceval_w (N, V, (l;;c)) (o::nil) (N', V', c) W
-   (*IP becomes obnoxious if you let checkpoint into the Seq case so I'm outlawing it
-    same with skip*)
-   (*ask arthur why sometimes it finds errors at the end before errors at the front*)
-| If_T: forall(N: nvmem)
-         (V: vmem)
-         (e: exp)
-         (r: readobs)
-         (c1 c2: command),
-    eeval N V e r true -> (*yuh doy not writing anything in eeval*)
-    cceval_w (N, V, (TEST e THEN c1 ELSE c2)) ((Obs r)::nil) (N, V, c1) (nil, (readobs_wvs r), nil)
-| If_F: forall(N: nvmem)
-         (V: vmem)
-         (e: exp)
-         (r: readobs)
-         (c1 c2: command),
-    eeval N V e r false ->
-    cceval_w (N, V, (TEST e THEN c1 ELSE c2)) ((Obs r)::nil) (N, V, c2) (nil, (readobs_wvs r), nil).
 
-Definition append_write (W1 W2: the_write_stuff) :=
-  ((getwt W2) ++ (getwt W1) , (getrd W2) ++ (getrd W1),  (remove (getrd W1) (getfstwt W2))
-                                         ++ (getfstwt W1)).
-(************************************************************)
+(*lemmas from paper*)
 
-(**********intermittent execution semantics*************************)
-(*evaluation relation for commands*)
-(*accumlates write data as continuous relation does*)
-Inductive iceval_w: iconf -> obseq -> iconf -> the_write_stuff -> Prop :=
-  CP_PowerFail: forall(k: context) (N: nvmem) (V: vmem) (c: command),
-    c <> (Ins skip) -> (*can't have a power fail if you've terminated*)
-                 iceval_w (k, N, V, c)
-                        nil
-                        (k, N, (reset V), Ins inreboot) (nil, nil, nil)
- | CP_Reboot: forall(N N': nvmem) (*see below*) (*N is the checkpointed one*)
-               (V V': vmem) 
-               (c: command),
-     c <> Ins inreboot ->
-     iceval_w ((N, V, c), N', V', Ins inreboot)
-            [:: reboot]
-            ((N, V, c), (N U! N'), V, c) (nil, nil, nil)
- | CP_CheckPoint: forall(k: context) (N: nvmem) (V: vmem) (c: command) (w: warvars),
-                 iceval_w (k, N, V, ((incheckpoint w);;c))
-                        [:: checkpoint]
-                        (((N |! w), V, c), N, V, c) (nil, nil, nil) 
- | CP_NV_Assign: forall(k: context) (x: smallvar) (N: nvmem) (V: vmem) (e: exp) (r: readobs) (v: value),
-    eeval N V e r v ->
-    isNV(x) -> (*checks x is correct type for NV memory*)
-    (isvaluable v) -> (*extra premise to check if v is valuable*)
-    iceval_w (k, N, V, Ins (asgn_sv x e))
-           [:: Obs r]
-           (k, (updateNV_sv N x v), V, Ins skip)
-           ([:: inl x],  (readobs_wvs r), (remove (readobs_wvs r) [:: inl x]))
-| CP_V_Assign: forall(k: context) (x: smallvar) (N: nvmem) (mapV: mem) (e: exp) (r: readobs) (v: value),
-    eeval N (Vol mapV) e r v ->
-    isV(x) -> (*checks x is correct type for V memory*)
-    (isvaluable v) -> (*extra premise to check if v is valuable*)
-    iceval_w (k, N, (Vol mapV), Ins (asgn_sv x e))
-           [:: Obs r]
-           (k, N, (Vol ((inl x) |-> v ; mapV)), Ins skip)
-             (nil,  (readobs_wvs r), nil)
-| CP_Assign_Arr: forall (k: context) (N: nvmem) (V: vmem)
-               (a: array)
-               (ei: exp)
-               (ri: readobs)
-               (vi: value)
-               (e: exp)
-               (r: readobs)
-               (v: value)
-               (element: el_loc),
-    eeval N V ei ri vi ->
-    eeval N V e r v ->
-    equal_index element a vi ->
-    (isvaluable v) -> (*extra premise to check if v is valuable*)
-    iceval_w (k, N, V, Ins (asgn_arr a ei e))
-           [:: Obs (ri++r)]
-           (k, (updateNV_arr N element a v), V, Ins skip)
-           ((generate_locs a), (readobs_wvs (cat r ri)), (remove  (readobs_wvs (cat r ri)) (generate_locs a)))
-| CP_Skip: forall(k: context) (N: nvmem)
-         (V: vmem)
-         (c: command),
-    iceval_w (k, N, V, (skip;;c)) ((Obs NoObs)::nil) (k, N, V, c) (nil, nil, nil)
-|CP_Seq: forall (k: context)
-         (N: nvmem) (N': nvmem)
-         (V: vmem) (V': vmem)
-         (l: instruction)
-         (c: command)
-         (o: obs)
-         (W: the_write_stuff),
-    (forall(w: warvars), l <> (incheckpoint w)) ->
-    l <> skip ->
-    iceval_w (k, N, V, Ins l) (o::nil) (k, N', V', Ins skip) W ->
-    iceval_w (k, N, V, (l;;c)) (o::nil) (k, N', V', c) W (*ask arthur like with those two os just there*)
-|CP_If_T: forall(k: context) (N: nvmem) (V: vmem)
-         (e: exp)
-         (r: readobs)
-         (c1 c2: command),
-    eeval N V e r true -> 
-    iceval_w (k, N, V, (TEST e THEN c1 ELSE c2)) ((Obs r)::nil) (k, N, V, c1) (nil, (readobs_wvs r), nil)
-|CP_If_F: forall(k: context) (N: nvmem) (V: vmem)
-         (e: exp)
-         (r: readobs)
-         (c1 c2: command),
-    eeval N V e r false ->
-    iceval_w (k, N, V, (TEST e THEN c1 ELSE c2)) ((Obs r)::nil) (k, N, V, c2) (nil, (readobs_wvs r), nil).
-(*CP_Reboot: I took out the equals premise and instead built it
-into the types because I didn't wanit to define a context equality function*)
+Lemma onePointone: forall(N N' W W' R R': warvars) (l: instruction),
+    DINO_ins N W R l N' W' R' -> subseq N N'.
+Proof. intros. induction H; try((try apply subseq_tl); apply (subseq_refl N)).
+       apply (subseq_cons N (inl x)).
+       apply suffix_subseq.
+Qed.
 
-(**************************************i******)
-(*helpers that use the evals
-Definition el_arrayexp_eq (e: el) (a: array) (eindex: exp) (N: nvmem) (V: vmem) := (*transitions from el type to a[exp] representation*)
-  (samearray e a) /\
-  exists(r: readobs) (vindex: value), eeval N V eindex r vindex /\
-                                 (eq_value (getindexel e) vindex).*)
-(******)
 
-(*ask arthur how to check in*)
-Close Scope type_scope.
+Lemma onePointtwo: forall(N N' W R: warvars) (c c': command),
+    DINO N W R c c' N' -> subseq N N'.
+Proof. intros. induction H; try(apply onePointone in H); try apply (incl_refl N); try assumption.
+       -  apply (subseq_trans H IHDINO).
+       - apply subseq_app_rr. assumption. apply subseq_refl.
+ Qed.
+
+Lemma Two: forall(N N' W W' R R' N1: warvars) (l: instruction),
+    DINO_ins N W R l N' W' R' -> subseq N' N1 -> WAR_ins N1 W R l W' R'.
+  intros. induction H; try ((constructor; assumption) || (apply War_noRd; assumption)).
+            (apply WAR_Checkpointed);
+              (repeat assumption).
+            move / in_subseq : H0.
+            intros.
+            apply (H0 (inl x) (mem_head (inl x) N)).
+            apply WAR_Checkpointed_Arr; try assumption. apply (subseq_app_l H0).
+
+Qed.
+
+
+Theorem DINO_WAR_correct: forall(N W R N': warvars) (c c': command),
+    DINO N W R c c' N' -> (forall(N1: warvars), subseq N' N1 -> WARok N1 W R c').
+  intros N W R c c' N' H. induction H; intros N0 Hincl.
+  - eapply WAR_I. applys Two H Hincl.
+  - eapply WAR_Seq. applys Two H. apply onePointtwo in H0.
+    apply (subseq_trans H0 Hincl).
+    apply (IHDINO N0 Hincl).
+  - eapply WAR_If; (try eassumption);
+      ((apply IHDINO1; apply subseq_app_l in Hincl)
+       || (apply IHDINO2; apply subseq_app_r in Hincl)); assumption.
+  - intros. apply WAR_CP. apply IHDINO. apply (subseq_refl N').
+Qed.
+
+
+Lemma eight: forall{N0 N1 N2: nvmem} {V0: vmem} {c0: command},
+              (subset_nvm N0 N1) ->
+              (subset_nvm N0 N2) ->
+              current_init_pt N0 V0 c0 N1 N1 N2 ->
+              same_pt N1 V0 c0 c0 N1 N2.
+Proof. intros. inversion H1. subst.
+ apply (same_mem
+                (CTrace_Empty (N1, V0, c0))
+                T); auto. 
+       - intros l Hl. simpl.
+        assert (H6: not (l \in (getdomain N0))) by
+               apply (sub_disclude N0 N1 N2 l H H0 Hl).
+         (*try appldis here*)
+         apply H5 in Hl. destruct Hl.
+         split.
+         + apply (in_subseq (wt_subst_fstwt T) H7).
+         + split. unfold remove. simpl.
+           rewrite filter_predT. rewrite cats0. assumption.
+             - intros contra. discriminate contra. 
+         + apply H6 in H7. contradiction.
+Qed.
+
+
+
+(*Concern: bottom three cases are essentially the same reasoning but with slight differences;
+ unsure how to automate
+ maybe remembering c so that I can use c instead of the specific form of c?*)
+(*N0 is checkpointed variables*)
+Lemma ten: forall(N0 W R: warvars) (N N': nvmem) (V V': vmem)
+            (O: obseq) (c c': command),
+            WARok N0 W R c ->
+            multi_step_c (N, V, c) (N', V', c') O ->
+            not (checkpoint \in O) ->
+            exists(W' R': warvars), WARok N0 W' R' c'.
+   intros.
+  generalize_5 N N' V V' O.
+  remember H as warok. clear Heqwarok.
+  induction H; intros.
+  +  destruct H0 as [ Wr T ].
+    cut (c' = Ins l \/ c' = skip).
+  - intros Hdis. destruct Hdis as [Hins | Hskip]; subst; exists W R.
+    + apply warok.
+    + eapply WAR_I. apply WAR_Skip.
+  - apply trace_stops in T. assumption.
+  + intros. destruct H0 as [ WT T ]. remember T as T1. clear HeqT1.
+        apply observe_checkpt in T. destruct T as [eq | contra].
+    - subst. exists W R. apply warok.
+    - apply H1 in contra. contradiction.
++ destruct H2 as [ WT T ]; subst.
+      assert (Dis: (l ;; c) = c' \/ not ((l;;c) = c'))
+          by (apply classic). destruct Dis.
+    - subst. exists W R. assumption.
+    - assert(exists(Csmall: context) (Osmall: obseq) (Wsmall: the_write_stuff),
+                  cceval_w (N0, V, l;;c) Osmall Csmall Wsmall).
+      + eapply trace_steps. apply T. intros contra. subst.
+        apply empty_trace in T. destruct T as [H3 H4].
+        inversion H3. apply H2. assumption. reflexivity.
+        destruct H3 as [Csmall rest].
+        destruct rest as [Osmall rest]. destruct rest as [Wsmall c1].
+        remember Csmall as Csmall1.
+        destruct Csmall as [blah1 smallcom]. destruct blah1 as [Nsmall Vsmall].
+        remember c1 as c11. clear Heqc11.
+        apply seq_step in c11. unfold getcom in c11. subst.
+        cut (exists(Wrest: the_write_stuff) (Orest: obseq), 
+                                                         trace_c
+                                                            (Nsmall, Vsmall, smallcom)
+                                                            (N', V', c')
+                                                            Orest Wrest
+                                                       /\ subseq Orest O).
+        move => [Wrest [ Orest [Tsmall inclO] ] ].
+        assert (Hmulti: multi_step_c
+              (Nsmall, Vsmall, smallcom)
+              (N', V', c') Orest) by (exists Wrest; assumption).
+        eapply IHWARok; try assumption.
+        + intros contra. apply (in_subseq inclO) in contra. apply H1 in contra. contradiction.
+          apply Hmulti.                          
+        + eapply single_step_all. apply T.
+      - intros contra. apply (empty_trace T) in contra. destruct contra as
+            [contra blah]. inversion contra. subst. apply H2. reflexivity.
+        exists Osmall Wsmall. assumption.
+ + destruct H3 as [WT T]; subst. remember (TEST e THEN c1 ELSE c2) as bigif.
+   assert (Dis: bigif = c' \/
+                bigif <> c')
+     by (apply classic). destruct Dis.
+      - subst. exists W R. apply warok.
+      - assert(exists(Csmall: context) (Osmall: obseq) (Wsmall: the_write_stuff),
+                  cceval_w (N0, V, bigif) Osmall Csmall Wsmall).
+        + eapply trace_steps. apply T. intros contra. subst.
+          apply empty_trace in T. destruct T as [H10 H11]. inversion H10. apply H3. assumption. reflexivity.
+        destruct H4 as [Csmall rest].
+        destruct rest as [Osmall rest]. destruct rest as [Wsmall cc].
+        remember Csmall as Csmall1.
+        destruct Csmall as [blah1 smallcom]. destruct blah1 as [Nsmall Vsmall].
+        remember cc as cc1. clear Heqcc1. rewrite Heqbigif in cc1.
+        apply if_step in cc1. destruct cc1 as [tcase | fcase].
+        - unfold getcom in tcase. subst.
+        cut (exists(Wrest: the_write_stuff) (Orest: obseq), 
+                                                         (trace_c
+                                                            (Nsmall, Vsmall, smallcom)
+                                                            (N', V', c')
+                                                            Orest Wrest)
+                                                       /\ subseq Orest O).
+        move => [Wrest [ Orest [Tsmall inclO] ] ].
+        assert (Hmulti: multi_step_c
+              (Nsmall, Vsmall, smallcom)
+              (N', V', c') Orest) by (exists Wrest; assumption).
+        eapply IHWARok1; try assumption.
+        + intros contra. apply (in_subseq inclO) in contra. apply H2 in contra. contradiction.
+          apply Hmulti.                          
+        + eapply single_step_all. apply T.
+      - intros contra. apply (empty_trace T) in contra. destruct contra as
+            [contra blah]. inversion contra. subst. apply H3. reflexivity.
+        exists Osmall Wsmall. assumption.
+      - unfold getcom in fcase. subst.
+        cut (exists(Wrest: the_write_stuff) (Orest: obseq), 
+                                                         (trace_c
+                                                            (Nsmall, Vsmall, smallcom)
+                                                            (N', V', c')
+                                                            Orest Wrest)
+                                                       /\ subseq Orest O).
+        move => [Wrest [ Orest [Tsmall inclO] ] ].
+        assert (Hmulti: multi_step_c
+              (Nsmall, Vsmall, smallcom)
+              (N', V', c') Orest) by (exists Wrest; assumption).
+        eapply IHWARok2; try assumption.
+        + intros contra. apply (in_subseq inclO) in contra. apply H2 in contra. contradiction.
+          apply Hmulti.                          
+        + eapply single_step_all. apply T.
+      - intros contra. apply (empty_trace T) in contra. destruct contra as
+            [contra blah]. inversion contra. subst. apply H3. reflexivity.
+        exists Osmall Wsmall. assumption.
+Qed.
+
+(*if trace from N1,c  to CP
+ then trace from N1' U! N0, c to CP
+ and indeed should be the SAME cp
+with same memories?
+yes as if diff in one of the mems, that diff came from a first accessed (in c)
+diff between N1 and (N1' U! N0). this diff is x. 
+at the start.
+case: x is not in CP.
+then, N1(x) != N1'(x). Since N1 --> N1' while doing c!,
+x was modified on the way to N1' while executing c.
+N1' = (N1 with x --> e).
+If x was read from before this point while executing c, then x would be in the CP by warok.
+So, x was not read from.
+So, when going the second time around from c, N1' does x --> e.
+Since x is the first diff
+
+Moreover, the expression x := e that x was assigned to must be equal in both cases, since
+N1 and (N1' U! N0) have been equal up until x  
+
+and that first diff existed between _whichever one_ and N2...not true, maybe theyre ALL different
+which means either it's a FW
+or in the CP ....but N1 isn't updated w a CP.... need subset relation?
+ but I don't need that just yet
+but i do need to show that the write sets are the same
+easiest way to do that might be to show everything the same?*)
+
+(*ask arthur is this supported by finite domain
+ type*)
+Lemma update_sub: forall{N0 N1: nvmem},
+    subset_nvm N0 N1 ->
+    (N0 U! N1) = N1.
+  intros. destruct N0, N1. unfold updatemaps.
+  Admitted.
+   (* need functionalextensionality here
+     also need to remove duplicates from the appending
+     so that this actually holds
+     only used in 12.1 so not gonna worry about it for now
+ i think the strat is to not use nodups and isntead do
+ ++ (remove D1 D0) removing D1 from D0 before appending*)
+
+Lemma sub_update: forall(N0 N1: nvmem),
+    subset_nvm N0 (N0 U! N1).
+  intros.
+  destruct N0, N1.
+  unfold subset_nvm. split.
+  simpl. apply prefix_subseq.
+  intros. simpl. by rewrite H.
+  Qed.
+
+(*ask arthur how does inversion not cover this*)
+Lemma stupid: forall (c: command) (l: instruction),
+    c <> (l ;; c).
+  move => c w contra.
+  induction c; inversion contra.
+    by apply IHc.
+Qed.
+
+
+(*the two below are taken for granted by the "configurations always make progress"
+ assumption, admitting it now, intend to fix it later*)
+
+(*termination case*)
+Lemma twelve00: forall{N0 N1 N1' NT: nvmem} {V V' VT: vmem} {c c': command} {O1 OT: obseq}
+  {WT: the_write_stuff},
+   multi_step_i ((N0, V, c), N1, V, c) ((N0, V, c), N1', V', c') O1
+      -> (checkpoint \notin O1)
+      -> WARok (getdomain N0) [::] [::] c
+      -> subset_nvm N0 N1
+      -> trace_c (N1, V, c) (NT, VT, Ins skip) OT WT
+      -> (checkpoint \notin OT)
+      -> trace_c ((N0 U! N1'), V, c) (NT, VT, Ins skip) OT WT.
+Admitted.
+
+(*checkpoint case*)
+Lemma twelve01: forall(N0 N1 N1' NCP: nvmem) (V V' VCP: vmem) (c c' cCP: command) (w: warvars) (O1 OCP: obseq)
+  (WCP: the_write_stuff),
+   multi_step_i ((N0, V, c), N1, V, c) ((N0, V, c), N1', V', c') O1
+      -> (checkpoint \notin O1)
+      -> WARok (getdomain N0) [::] [::] c
+      -> subset_nvm N0 N1
+      -> trace_c (N1, V, c) (NCP, VCP, (incheckpoint w);; cCP) OCP WCP
+      -> (checkpoint \notin OCP)
+      -> trace_c ((N0 U! N1'), V, c) (NCP, VCP, (incheckpoint w);; cCP) OCP WCP.
+  (*intros. rename H3 into T.
+  destruct_ms H Ti WTi.
+  dependent induction Ti. (*makes a diff here w remembering that N1 and N1' are the same*)
+  + rewrite (update_sub H2).  assumption.
+  + dependent induction i.
+     - rewrite (update_sub H2). assumption.
+     - repeat rewrite (update_sub H2).  assumption. 
+     - exfalso. eapply stupid in x. contradiction.
+     - 
+       above might be a little broken bc you changed from type
+        to prop w/o checking*)
+       (*x has been written to
+  unfold multi_step_c in H.
+  destruct H.*)
+
+Admitted.
+
+Lemma dom_gets_bigger_rb: forall(N0 N1: nvmem),
+    subseq (getdomain N1) (getdomain (N0 U! N1)).
+  move => [m0 d0] [m1 d1]. simpl. apply suffix_subseq.
+  Qed.
+
+Lemma dom_gets_bigger: forall{N1 N1': nvmem} {V V': vmem} {k0 k1: context}
+                        {c c': command} {O: obseq},
+      multi_step_i (k0, N1, V, c) (k1, N1', V', c') O ->
+   subseq (getdomain N1) (getdomain N1').
+  intros. destruct H as [w T].
+  dependent induction T.
+  apply subseq_refl.
+  dependent induction H; try (apply subseq_refl); try
+                                                    apply dom_gets_bigger_rb.
+  destruct N1. unfold updateNV_sv. unfold getdomain.
+ apply (subseq_cons D (inl x)). 
+  destruct N1. unfold updateNV_arr. unfold getdomain.
+  apply (suffix_subseq (generate_locs a) D).
+  eapply IHiceval_w; (try reflexivity).
+  destruct Cmid as [ [ [ Kmid Nmid ] Vmid ] cmid].
+  eapply subseq_trans; [eapply IHT1 | eapply IHT2]; try reflexivity.
+Qed.
+
+Lemma updateone_sv: forall{N: nvmem} {x: smallvar} {v: value}
+             {l: loc},
+    not (((getmap (updateNV_sv N x v)) l) = ((getmap N) l) ) ->
+               (l = (inl x)).
+  intros.
+  destruct (l == inl x) eqn: beq.
+  apply/ eqP : beq.
+  destruct N as [M D].
+  unfold updateNV_sv in H.
+  simpl in H.
+  unfold updatemap in H.
+  rewrite beq in H.
+  exfalso. by apply H. 
+  Qed.
+
+Lemma updateone_arr: forall{N: nvmem} {a: array} {v: value}
+             {i: el_loc} {l: loc},
+    not (((getmap (updateNV_arr N i a v)) l) = ((getmap N) l) ) ->
+               (l = (inr i)).
+  intros.
+  destruct (l == inr i) eqn: beq.
+  apply/ eqP : beq.
+  destruct N as [M D].
+  unfold updateNV_arr in H.
+  simpl in H.
+  unfold updatemap in H.
+  rewrite beq in H.
+  exfalso. by apply H. 
+  Qed.
+
+Lemma update_one: forall{N N0 Nend: nvmem} {V V0 Vend: vmem} {c c0 cend: command} {O: obseq} {W: the_write_stuff}
+  {l: loc},
+    iceval_w ((N0, V0, c0), N, V, c) O ((N0, V0, c0), Nend, Vend, cend) W ->
+    (getmap N) l <> (getmap Nend) l ->
+    reboot \notin O ->
+    l \in (getwt W).
+  intros.
+  dependent induction H; try (exfalso; by (apply H0 ||
+                             apply H2)); simpl.
+(*start here use ssreflect to fix this garbage*)
+  apply not_eq_sym in H2.
+  apply updateone_sv in H2.
+  subst. by rewrite mem_seq1.
+  (*move/ not_eq_sym : H3.
+   ask arthur why is this not cooperating*)
+  apply not_eq_sym in H3.
+  apply updateone_arr in H3.
+  subst. destruct element. by pose proof (gen_locs_works H1).
+  eapply IHiceval_w; try reflexivity; try
+  assumption.
+  Qed.
+
+Lemma iceval_cceval: forall{k: context} {N Nend1 Nend2 : nvmem} {V Vend1 Vend2: vmem}
+                      {c cend1 cend2 : command} {O1 O2: obseq} {W1 W2: the_write_stuff},
+    iceval_w (k, N, V, c) O1 (k, Nend1, Vend1, cend1) W1 ->
+    cceval_w (N, V, c) O2 (Nend2, Vend2, cend2) W2 ->
+    (Nend1 = N /\ Vend1 = (reset V) /\ W1 = emptysets /\ cend1 = Ins inreboot) \/
+    (Nend1 = Nend2 /\ Vend1 = Vend2 /\ W1 = W2).
+  intros.
+  move : cend2 H0.
+  dependent induction H; intros.
+  left. (*do! [split]. by [].*)
+  split; [reflexivity | split; [reflexivity | split; reflexivity] ].
+  inversion H0.
+  inversion H0; subst. right.
+  split; [reflexivity | split; reflexivity ].
+  exfalso. by apply (H9 w).
+  inversion H2; subst. right.
+  destruct (determinism_e H H12). subst.
+  split; [reflexivity | split; reflexivity ].
+  exfalso. apply (negNVandV x H0 H13).
+inversion H2; subst. right.
+exfalso. apply (negNVandV x H13 H0).
+right.
+  destruct (determinism_e H H12). subst.
+  split; [reflexivity | split; reflexivity ].
+  right.
+  inversion H3; subst.
+  destruct (determinism_e H H14).
+  destruct (determinism_e H0 H15).
+  subst.
+  pose proof (equal_index_works H16 H1).
+  subst.
+  split; [reflexivity | split; reflexivity ].
+  right. inversion H0; subst.
+  split; [reflexivity | split; reflexivity ].
+  exfalso. by apply H10.
+  inversion H2; subst.
+  - exfalso. by apply (H w).
+  - exfalso. by apply H0.
+    suffices:
+  (Nend1 = N /\
+  Vend1 = reset V /\ W = ([::], [::], [::]) /\ Ins skip = Ins inreboot \/
+   Nend1 = Nend2 /\ Vend1 = Vend2 /\ W = W2).
+    intros. right.
+    destruct x as [ [ contraN [ contraV [contraW contrac] ] ] | H5 ].
+    discriminate contrac. assumption.
+    eapply IHiceval_w; try reflexivity.
+    apply H14.
+    right. inversion H0; subst;
+    destruct (determinism_e H H11); subst.
+    split; [reflexivity | split; reflexivity ].
+    inversion H2.
+    right. inversion H0; subst;
+    destruct (determinism_e H H11); subst.
+    inversion H2.
+    split; [reflexivity | split; reflexivity ].
+(*ask arthur how to do a recursive tactic
+ for dealing with big conjunctions*)
+Qed.
+
+Lemma cceval_iceval: forall {N Nend : nvmem} {V Vend: vmem}
+                      {c cend: command} {O: obseq} {W: the_write_stuff},
+    cceval_w (N, V, c) O (Nend, Vend, cend) W ->
+    (forall(k: context), iceval_w (k, N, V, c) O (k, Nend, Vend, cend) W).
+Admitted.
+
+  Lemma wt_gets_bigger: forall{N N0 N1 Nend: nvmem} {V V0 V1 Vend: vmem} {c c0 c1 cend: command} {O0 O1: obseq} {W0 W1: the_write_stuff}
+  {l: loc},
+    iceval_w ((N0, V0, c0), N, V, c) O0 ((N0, V0, c0), N1, V1, c1) W0 ->
+    trace_c (N, V, c) (Nend, Vend, cend) O1 W1 ->
+    O1 <> [::] ->
+    l \in (getwt W0) ->
+          l \in (getwt W1).
+  intros. dependent induction H0.
+  + exfalso. by apply H1.
+  + pose proof (iceval_cceval H H0).
+    destruct H3 as [ [ contraN [ contraV [contraW contrac] ] ]  | [ Hn [ Hv Hw ] ] ]; subst.
+    rewrite in_nil in H2. discriminate H2. assumption.
+    destruct W1 as [ [w1 rd1] fw1].
+    destruct W2 as [ [w2 rd2] fw2].
+    simpl.
+    rewrite mem_cat.
+    apply (introT orP). right.
+    destruct3 Cmid nmid vmid cmid.
+    eapply IHtrace_c1; try
+                         apply H; try reflexivity; try assumption.
+Qed.
+Lemma read_deterministic: forall{e: exp} {w1 w2: warvars},
+                           rd e w1 ->
+                           rd e w2 ->
+                           w1 = w2.
+  intros.
+ inversion H. inversion H0. subst. 
+  move: H0 H4. move: N0 V0 rs0 v0. dependent induction H1; intros.
+  + by inversion H4.
+  + inversion H4; subst. apply IHeeval1 in H8;
+                           
+                           apply IHeeval2 in H11;
+                        try(   rewrite (readobs_app_wvs r1 r2);
+    rewrite (readobs_app_wvs r0 r3);
+      by rewrite H8 H11);
+                        try ( eapply RD; (apply H11) || (apply H1_0) || (apply H1_)
+                            || (apply H8)).
+  + simpl. inversion H4; subst; simpl; auto.
+  + simpl. inversion H4; subst; simpl; auto.
+  + inversion H5. subst. rewrite (readobs_app_wvs rindex).
+    rewrite (readobs_app_wvs rindex0).
+    suffices: (readobs_wvs rindex) =(readobs_wvs rindex0).
+    move ->.
+    destruct element. destruct element0.
+ pose proof (equal_index_arr H2) as arreq. 
+ pose proof (equal_index_arr H12) as arreq1. by subst.
+ eapply IHeeval. apply (RD H1).
+ apply (RD H8). apply H8.
+Qed.
+
+
+Lemma negfwandw_means_r: forall{C Cend: context}  {O: obseq} {W: the_write_stuff}
+  {l: loc},
+    trace_c C Cend O W ->
+    l \notin (getfstwt W) -> l \in (getwt W) -> l \in (getrd W).
+  intros. destruct3 W w rD fw.
+  dependent induction H.
+  + discriminate H1.
+  + induction H; (try discriminate H1);
+    simpl in H1;
+    simpl in H0;
+    simpl.
+    destruct (l \in readobs_wvs r) eqn: beq.
+    auto.
+    apply negbT in beq.
+    rewrite mem_seq1 in H1.
+    move/eqP: H1 => H1. subst.
+    rewrite beq in H0.
+    rewrite mem_seq1 in H0.
+    move/eqP: H0 => contra.
+    exfalso. by apply contra.
+    destruct (l \in readobs_wvs (r ++ ri)) eqn: beq.
+    auto.
+    rewrite mem_filter in H0.
+    move/ nandP : H0 => [contra1 | contra2].
+           + by move/ negPn : contra1.
+           + rewrite H1 in contra2. discriminate contra2.
+    apply IHcceval_w; assumption.
+    destruct W1 as [ [w1 rd1] fw1].
+    destruct W2 as [ [w2 rd2] fw2].
+    simpl in H3. simpl in H4.
+    simpl.
+    simpl in IHtrace_c1.
+    simpl in IHtrace_c2.
+    rewrite mem_cat.
+    apply (introT orP).
+    rewrite mem_cat in H3.
+    case/norP : H3 => [H32 H31].
+    rewrite mem_cat in H4.
+    move/ orP : H4 => [H40 | H41].
+  + destruct (l \in rd1) eqn: beq1.
+    - auto.
+      left.
+      rewrite mem_filter in H32.
+      move/ nandP : H32 => [H320 | H321].
+      rewrite beq1 in H320.
+     move/negPn : H320 => contra.
+      discriminate contra.
+    - eapply IHtrace_c2; try reflexivity;
+        try assumption.
+  + right. eapply IHtrace_c1; try
+                               reflexivity; try assumption.
+ Qed.
+
+Lemma cceval_to_rd_sv: forall {N Nend: nvmem} {V Vend: vmem}
+                      {e: exp} {x: smallvar} {O: obseq}
+                      {W: the_write_stuff}
+                      {Re: warvars}
+  {cend: command},
+    cceval_w (N, V, Ins (asgn_sv x e)) O
+        (Nend, Vend, cend) W ->
+    rd e Re ->
+    (getrd W) = Re.
+  intros.
+  inversion H; subst; try(
+                          pose proof (read_deterministic H0 (RD H10)); by subst).
+Qed.
+
+Lemma extract_write_svnv: forall {N Nend: nvmem} {V Vend: vmem}
+                      {e: exp} {x: smallvar} {O: obseq}
+                      {W: the_write_stuff}
+  {cend: command},
+    cceval_w (N, V, Ins (asgn_sv x e)) O
+             (Nend, Vend, cend) W ->
+    (isNV x) ->
+    (getwt W) = [:: inl x].
+  intros.
+  inversion H; subst; try reflexivity.
+  exfalso. apply (negNVandV x H0 H11).
+Qed.
+
+Lemma extract_write_svv: forall {N Nend: nvmem} {V Vend: vmem}
+                      {e: exp} {x: smallvar} {O: obseq}
+                      {W: the_write_stuff}
+  {cend: command},
+    cceval_w (N, V, Ins (asgn_sv x e)) O
+             (Nend, Vend, cend) W ->
+    (isV x) ->
+    (getwt W) = [:: ].
+  intros.
+  inversion H; subst; try reflexivity.
+  exfalso. apply (negNVandV x H11 H0).
+Qed.
+
+Lemma extract_write_arr: forall {N Nend: nvmem} {V Vend: vmem}
+                      {e ei: exp} {a: array} {O: obseq}
+                      {W: the_write_stuff}
+  {cend: command},
+    cceval_w (N, V, Ins (asgn_arr a ei e)) O
+             (Nend, Vend, cend) W ->
+   (getwt W) = (generate_locs a).
+  intros.
+  inversion H; subst.
+   reflexivity.
+Qed.
+
+(*probs should have inducted over
+ cceval instead of warok below, clean up*)
+Lemma war_cceval: forall{N0 N Nmid: nvmem} {V Vmid: vmem} {c cmid: command}
+                   {l: instruction}
+                   {O: obseq} {W: the_write_stuff} {Wstart Rstart W' R': warvars},
+
+        cceval_w (N, V, l;;c) O (Nmid, Vmid, cmid) W ->
+        WAR_ins (getdomain N0) Wstart Rstart l W' R' ->
+        ( W' = (getwt W) ++ Wstart) /\ (R' =  (getrd W) ++ Rstart).
+  intros. dependent induction H0.
+  - (*skip case*) inversion H; subst. split; reflexivity.
+    exfalso. by apply H10.
+  - inversion H; subst. pose proof (extract_write_svv H14 H0).
+    rewrite H3. inversion H14; subst;
+    pose proof (read_deterministic H2 (RD H15));
+    subst; split; reflexivity. (*vol case*)
+ - inversion H; subst. pose proof (extract_write_svnv H14 H2).
+    rewrite H3. inversion H14; subst;
+    pose proof (read_deterministic H0 (RD H15));
+    subst; split; reflexivity. (*nord case*)
+ -inversion H; subst. pose proof (extract_write_svnv H16 H0).
+    rewrite H5. inversion H16; subst;
+    pose proof (read_deterministic H4 (RD H17));
+    subst; split; reflexivity. (*CP case*)
+ - inversion H; subst. pose proof (extract_write_svnv H15 H2).
+    rewrite H4. inversion H15; subst;
+    pose proof (read_deterministic H3 (RD H16));
+    subst; split; reflexivity. (*written to case*)
+ - (*nrd arr case*) inversion H; subst; inversion H14; subst. simpl. rewrite readobs_app_wvs. rewrite catA.
+   pose proof (read_deterministic H2 (RD H16)).
+   pose proof (read_deterministic H0 (RD H15)).
+   subst. split; reflexivity.
+ - inversion H; subst; inversion H15; subst. simpl. rewrite readobs_app_wvs. rewrite catA.
+   pose proof (read_deterministic H3 (RD H17)).
+   pose proof (read_deterministic H0 (RD H16)).
+   subst. split; reflexivity.
+Qed.
+
+
+
+Lemma cceval_steps: forall{N Nmid: nvmem} {V Vmid: vmem} {c cmid: command}
+                   {O: obseq} {W: the_write_stuff} {l: instruction},
+
+        cceval_w (N, V, l;;c) O (Nmid, Vmid, cmid) W ->
+        c = cmid.
+intros. inversion H; subst; try reflexivity. Qed.
+
+
+Lemma cceval_steps_ins: forall{N Nmid: nvmem} {V Vmid: vmem} {cmid: command}
+                   {O: obseq} {W: the_write_stuff} {l: instruction},
+
+        cceval_w (N, V, Ins l) O (Nmid, Vmid, cmid) W ->
+        cmid = Ins skip.
+intros. inversion H; subst; try reflexivity. Qed.
+(*doesn't this just follow immediately
+ from construction of W', R' in WARins?*)
+Lemma warok_partial:  forall{N0 N Nmid: nvmem} {V Vmid: vmem} {c cmid: command} {O: obseq} {W: the_write_stuff} {Wstart Rstart: warvars},
+    trace_c (N, V, c) (Nmid, Vmid, cmid) O W ->
+    checkpoint \notin O ->
+    WARok (getdomain N0) Wstart Rstart c ->
+    WARok (getdomain N0) ((getwt W) ++ Wstart) ((getrd W) ++ Rstart) cmid.
+  intros.
+  move: H1.
+  move : Wstart Rstart.
+  dependent induction H; intros.
+  + simpl.  assumption.
+    (*inducting warok
+    move: H H0.
+    move: cmid W N V Nmid Vmid O.*)
+    dependent induction H1.
+  - (*ins case, getting skip for last com of cceval*)
+    pose proof (cceval_steps_ins H). subst. eapply WAR_I. constructor.
+  - (*CP case*)
+    inversion H; subst.
+      - exfalso. rewrite mem_seq1 in H0. move/ eqP :H0.
+      by apply.
+      - exfalso. by apply (H11 w).
+  - (*seq case*) 
+    intros.
+    destruct (war_cceval H H2). subst.
+    pose proof (cceval_steps H). subst. assumption.
+  - (*if case*)
+    inversion H; subst; 
+    pose proof (read_deterministic H1 (RD H12));
+    subst; assumption.
+    (*inductive case trace*)
+    destruct3 Cmid nmid vmid cmiddle.
+    simpl.
+    repeat rewrite <- catA.
+    rewrite mem_cat in H3.
+    move/ norP : H3 => [H31 H32].
+    eapply IHtrace_c2; try reflexivity; try assumption.
+    eapply IHtrace_c1; try reflexivity; try assumption.
+Qed.
+    (*wts
+     W' = W0 ++ W
+     R' = R ++ getrd W0*)
+    (*inductive cceval step
+    inversion H3; subst.*)
+  (* - cp case exfalso. by apply (H w).
+    eapply IHcceval_w; try reflexivity.*)
+
+
+
+Lemma fourteen: forall{N0 N Nend: nvmem} {V Vend: vmem} {c cend: command} {O: obseq} {W: the_write_stuff}
+                  {Wstart Rstart: warvars} (l: loc),
+    trace_c (N, V, c) (Nend, Vend, cend) O W ->
+    WARok (getdomain N0) Wstart Rstart c ->
+    checkpoint \notin O ->
+    (*O <> [::] -> empty trace annoying and i dont think
+               i have to deal w it*)
+    l \notin (remove Rstart (getfstwt W)) -> (*l not in OVERALL FW for this trace*)
+    l \in (getwt W) -> (*l written to
+                       IN THIS trace*)
+    l \in (getdomain N0) \/ l \in Wstart. (*l is checkpointed
+                                          or l was already
+                                          written to
+                                          in which case can't
+                                          say*)
+  intros. move: Wstart Rstart H0 H1 H2 H3.
+  dependent induction H; intros. (*inducting on trace *)
+  + (*emoty trace*)
+    intros. rewrite in_nil in H3. discriminate H3. 
+  + (*single trace*)
+    move: H0 H1 H2 H3. move: Wstart Rstart.
+    remember H as H01. clear HeqH01.
+    dependent induction H01; intros;
+      try (rewrite in_nil in H3; discriminate H3);
+try (rewrite in_nil in H4; discriminate H4)
+    .
+    
+    (*inducting cceval*)
+  + (*nonvol case*)
+    (*showing x = l*)
+    remember H6 as Hwt. clear HeqHwt. 
+         simpl in H6.
+         rewrite mem_seq1 in H6.
+         move/ eqP : H6 => H6. subst.
+       inversion H3; subst; inversion H10;
+       subst. (*casing on warIns*)
+     (*vol case, x \notin getwt W*)
+       +  exfalso. apply (negNVandV x H0 H13).
+       + (*nord case*)
+         (*showing l in rd W*)
+
+         rewrite mem_cat in H16.
+         move / negP / norP : H16 => [H160 H161].
+         rewrite mem_filter in H5.
+         rewrite negb_and in H5.
+         simpl in H5.
+         rewrite H161 in H5.
+         rewrite orFb in H5.
+         pose proof (negfwandw_means_r (CTrace_Single H) H5 Hwt) as Hrd. simpl in Hrd.
+       (*showing x notin RD(W)*)
+       pose proof (read_deterministic H13 (RD H2)). subst. rewrite Hrd in H160. discriminate H160.
+     + (*CP case*)
+        by left.
+     + (*written case*)
+       by right.
+     - (*vol case*)
+       simpl in H6. rewrite in_nil in H6.
+       discriminate H6.
+     - (*array case*)
+    (*showing x = l*)
+       remember H7 as Hwt. clear HeqHwt.
+       simpl in H7.
+       simpl in H6.
+       (*  rewrite mem_seq1 in H7.
+         move/ eqP : H7 => H7. subst.*)
+       inversion H4; inversion H12;
+       subst. (*casing on warIns*)
+       + (*nord arr*)
+         (*showing l in rd W*)
+         suffices: (l \notin Rstart).
+         - intros Hstart.
+        (* rewrite mem_cat in H22.
+         move / negP / norP : H16 => [H160 H161].*)
+         rewrite mem_filter in H6.
+         rewrite negb_and in H6.
+         rewrite Hstart in H6.
+         rewrite orFb in H6.
+         pose proof (negfwandw_means_r (CTrace_Single H) H6 Hwt) as Hrd. simpl in Hrd.
+       (*showing x notin RD(W)*)
+       exfalso.
+       apply H23.
+       exists (l : loc).
+       split.
+       apply Hwt.
+       (*showing rd sets are same*)
+       pose proof
+            (read_deterministic (RD H0) H19).
+       pose proof
+            (read_deterministic (RD H3) H22).
+       subst.
+       rewrite catA.
+       rewrite <- readobs_app_wvs.
+       rewrite mem_cat.
+       apply (introT orP).
+       left.
+       apply Hrd.
+         - apply (introT negP).
+           intros contra. apply H23.
+           exists (l : loc).
+       split.
+       destruct element.
+       apply Hwt.
+       rewrite catA.
+       rewrite mem_cat.
+       apply (introT orP).
+      by right.
+     + (*CP array*)
+         destruct element.
+         pose proof (equal_index_arr H1). subst.
+         left.
+         apply (in_subseq H24 H7).
+ - (*seq case*)
+    eapply IHH01; try apply H01; try reflexivity; try assumption.
+    inversion H2; subst. (*invert WARok to get warins*)
+    + (*CP case warok*)
+    exfalso. by apply (H1 w).
+    + (*seq case warok*)
+      eapply WAR_I; apply H11; try assumption.
+      assumption.
+      (*clean up above*)
+    + (*trace inductive step*)
+simpl in H6. rewrite mem_cat in H6.
+destruct3 Cmid nmid vmid cmid.
+destruct (l \in (getwt W1)) eqn: beq.
+       + (*x written in 1st half*)
+         eapply IHtrace_c1; try reflexivity;
+           try assumption.
+         apply H3.
+         rewrite mem_cat in H4.
+         move/ norP : H4 => [H41 H42].
+         assumption.
+         simpl in H5.
+         apply (remove_app_r H5).
+     + (*2nd half, NOT in first half *)
+         rewrite mem_cat in H4.
+         move/ norP : H4 => [H41 H42].
+       suffices:
+         (is_true (l \in getdomain N0) \/ is_true (l \in (getwt W1) ++ Wstart)).
+          - move => [Case1 | Case2].
+          - by left.
+          - right. rewrite mem_cat in Case2.
+            move / orP : Case2 => [contra | yes].
+            - rewrite contra in beq. discriminate beq.
+            - assumption.
+       eapply IHtrace_c2; try reflexivity; try
+        apply (warok_partial H H41 H3); try
+                                          assumption.
+       unfold append_write in H5.
+       simpl in H5.
+       unfold remove in H5.
+       rewrite filter_cat in H5.
+       unfold remove.
+       rewrite mem_cat in H5.
+       move / norP : H5 => [H50 H51].
+       rewrite <- remove_to_app in H50.
+       assumption.
+       move/ orP : H6 => [H60 | H61].
+            - assumption.
+            - rewrite beq in H61. discriminate H61.
+Qed.
+
+
+Lemma pf_idem : forall(N0 N Nend: nvmem) (V0 V Vend: vmem)
+                      (c0 c: command) (O : obseq) (W : the_write_stuff),
+        iceval_w ((N0, V0, c0), N, V, c) O
+                 ((N0, V0, c0), Nend, Vend, c) W -> N = Nend.
+  intros.
+  dependent induction H; (try auto).
+  + exfalso. by apply H. (*here is where reboot case happens*)
+  + 
+    apply stupid in x. contradiction.
+ Qed.
+
+
+    Lemma fifteen: forall{N0 N1 N1' N2: nvmem} {V V': vmem} {c c': command} {O: obseq} {W: the_write_stuff},
+             iceval_w ((N0, V, c), N1, V, c) O
+             ((N0, V, c), N1', V', c') W ->
+             (checkpoint \notin O) ->
+             (reboot \notin O) ->
+             WARok (getdomain N0) [::] [::] c ->
+             current_init_pt N0 V c N1 N1 N2 ->
+             subset_nvm N0 N1 ->
+             current_init_pt N0 V c (N0 U! N1') (N0 U! N1') N2.
+  intros. inversion H3. subst. remember T as TN1. clear HeqTN1.
+  destruct H5; subst. (*casing on skip*)
+  +      eapply valid_mem.
+(*need to show N0 U! N1' can make it*)
+         - assert(trace_c ((N0 U! N1'), V, c) (Nend, Vend, Ins skip) O0 W0) as T2.
+           eapply twelve00.
+           (*recent ask arthur won't let me put a semicolon!
+           *)
+   exists W; try (apply (iTrace_Single H)). assumption.
+   assumption. assumption. assumption. assumption.
+     apply T2. by left.
+       - (*showing N2 subst N0 U! N1'
+          Ignore this bullet: I forgot to take out this part of the
+          relation after our last meeting*)
+assert (multi_step_i ((N0, V, c), N1, V, c)
+                              ((N0, V, c), N1', V', c') O).
+         exists W.  apply (iTrace_Single H).
+         apply (subseq_trans
+                  (subseq_trans H6 (dom_gets_bigger
+                                      H5)) (dom_gets_bigger_rb
+                                                    N0 N1')).
+         assumption.
+  (*casing on whether l is different in N1*)
+  intros. destruct (getmap N1 l == getmap N2 l) eqn: beq. (*casing on fw or not*)
+           move/eqP :beq => beq. rewrite <- beq in H5.
+           (*since they are equal but N1' is different on l, l
+            is not checkpointed*)
+           assert (not(l \in getdomain N0)).
+           unfold subset_nvm in H4. destruct H4 as [H41 H42].
+           intros contra. remember contra as contra1.
+           clear Heqcontra1. apply H42 in contra1.
+           destruct (sub_update N0 N1') as [blah HN1'].
+           apply HN1' in contra.
+           rewrite contra1 in contra.
+           symmetry in contra.
+           apply H5 in contra. contradiction.
+           destruct N0 as [M0 D0] eqn: N0eq.
+           destruct N1' as [M1' D1'] eqn: N1'eq.
+           assert (M1' = (getmap N1')) as rememberme.
+            by rewrite N1'eq. 
+           assert (D0 = (getdomain N0)) as rememberme1.
+             by rewrite N0eq.
+             remember N1'eq as stayput.
+             remember N0eq as stayput1.
+           unfold updatemaps in H5.
+           simpl in H5.
+           simpl in H9.
+           apply not_true_is_false in H9.
+           rewrite H9 in H5.
+           simpl.
+           (*now have that l is not in D0*)
+           left.
+(*inverting T to split up W0*)
+           inversion T; subst.
+           inversion H. subst.
+          exfalso. by apply H5.
+(*single trace case*)
++ destruct (iceval_cceval H H10) as [ [ HN [HV Hw] ] | [HN [HV Hw ] ] ]; subst.
+       - (*pf case*) exfalso. by apply H5.
+       - 
+  destruct W0 as [ [W11 R1] Fw1] eqn: W1eq.
+  simpl.
+         suffices: (l \in W11).
+         intros HW1.
+         destruct (l \in Fw1) eqn: FWeq; auto.
+         apply negbT in FWeq.
+         pose proof (negfwandw_means_r TN1 FWeq HW1) as Hr.
+         simpl in Hr.
+         suffices: (
+       is_true (l \in D0)
+                   ).
+         case => contra.
++ rewrite H9 in contra. discriminate contra.
+  rewrite rememberme1.
+  suffices: (is_true (l \in getdomain (NonVol M0 D0)) \/
+             is_true (l \in [::])).
+  - move => [yes | contra]. assumption.
+  rewrite in_nil in contra. discriminate contra.
+  -
+    apply (fourteen l TN1 H2); try assumption.
+    (*rewrite filter_predT.*)
+    rewrite remove_empty. assumption.
+         (*this comes from fact that N1 steps to M1'
+          in one (H) but N1 l and M1' of l are different.. new theorem*)
+         assert (W11 = (getwt W0)) as Hwt. by rewrite W1eq; auto.
+         rewrite Hwt.
+         eapply (wt_gets_bigger H).
+         rewrite <- W1eq in TN1.
+         apply TN1.
+         intros contra. subst.
+         inversion H10.
+         apply (update_one H); try assumption.
+         intros contra. apply H5.
+         rewrite rememberme. symmetry. assumption.
+(*larger trace case; exact same reasoning
+ significant potential for
+ decreasing boilerplate if I just proved
+ that fstwt set grows as trace gets bigger,
+ used first IH*)
++ destruct W1 as [ [W11 R1] Fw1] eqn: W1eq.
+         destruct W2 as [ [W22 R2] Fw2] eqn: W2eq.
+         unfold append_write.
+         simpl.
+         suffices: (l \in Fw1).
+         intros. rewrite mem_cat.
+         apply (introT orP). by right.
+         simpl in H8.
+         suffices: (l \in W11).
+         intros HW1.
+         destruct (l \in Fw1) eqn: FWeq; auto.
+         apply negbT in FWeq.
+         pose proof (negfwandw_means_r H10 FWeq HW1) as Hr.
+         simpl in Hr.
+         suffices: (is_true (l \in Fw1 ++ remove R1 Fw2) \/
+       is_true (l \in D0)
+                   ).
+         destruct (l \in Fw1 ++ remove R1 Fw2) eqn: deq.
+         rewrite mem_cat in deq.
+         move/ orP : deq.
+         case => Hin.
+          rewrite Hin in FWeq.
+         discriminate FWeq.
+         rewrite mem_filter in Hin.
+         case/ andP : Hin => [ contra blah ].
+         rewrite Hr in contra. discriminate contra.
+         case => contra.
+         assumption.
+         rewrite H9 in contra. assumption.
+         right. rewrite rememberme1.
+         destruct3 Cmid nmid vmid cmid.
+  suffices: (is_true (l \in getdomain (NonVol M0 D0)) \/
+             is_true (l \in [::])).
+  - move => [yes | contra]. assumption.
+  rewrite in_nil in contra. discriminate contra.
+  -
+    apply (fourteen l H10 H2); try (rewrite remove_empty);
+      try assumption.
+         rewrite mem_cat in H7.
+         case/ norP : H7 => Hor1 Hor2. assumption.
+         (*this comes from fact that N1 steps to M1'
+          in one (H) but N1 l and M1' of l are different.. new theorem*)
+         assert (W11 = (getwt W1)) as Hwt. by rewrite W1eq; auto.
+         rewrite Hwt.
+         destruct3 Cmid nmid vmid cmid.
+         eapply wt_gets_bigger.
+         apply H.
+         rewrite <- W1eq in H10.
+         apply H10.
+         assumption.
+         apply (update_one H); try assumption.
+         intros contra. apply H5.
+         rewrite rememberme. symmetry. assumption.
+(*N1 l != N2 l*)
++ apply H8. by move/ eqP : beq.
+
+ (*checkpoint case
+  consider doing the H5 casing later on so you have less boilerplate*)
+ + destruct H5 as [wcp [crem2 cpeq] ]. subst.
+   eapply valid_mem.
+     assert(trace_c ((N0 U! N1'), V, c) (Nend, Vend, incheckpoint wcp;;
+          crem2) O0 W0) as T2.
+eapply twelve01.
+   exists W. apply (iTrace_Single H). assumption.
+   assumption. assumption.  assumption. assumption.
+     apply T2. right. exists wcp crem2. reflexivity.
+       - (*showing N2 subst N0 U! N1'*)
+assert (multi_step_i ((N0, V, c), N1, V, c)
+                              ((N0, V, c), N1', V', c') O).
+         exists W.   apply (iTrace_Single H).
+         apply (subseq_trans
+                  (subseq_trans H6 (dom_gets_bigger
+                                      H5)) (dom_gets_bigger_rb
+                                                    N0 N1')).
+         assumption.
+  (*casing on whether l is different in N1*)
+  intros. destruct (getmap N1 l == getmap N2 l) eqn: beq. (*casing on fw or not*)
+           move/eqP :beq => beq. rewrite <- beq in H5.
+           (*since they are equal but N1' is different on l, l
+            is not checkpointed*)
+           assert (not(l \in getdomain N0)).
+           unfold subset_nvm in H4. destruct H4 as [H41 H42].
+           intros contra. remember contra as contra1.
+           clear Heqcontra1. apply H42 in contra1.
+           destruct (sub_update N0 N1') as [blah HN1'].
+           apply HN1' in contra.
+           rewrite contra1 in contra.
+           symmetry in contra.
+           apply H5 in contra. contradiction.
+           destruct N0 as [M0 D0] eqn: N0eq.
+           destruct N1' as [M1' D1'] eqn: N1'eq.
+           assert (M1' = (getmap N1')) as rememberme.
+            by rewrite N1'eq. 
+           assert (D0 = (getdomain N0)) as rememberme1.
+             by rewrite N0eq.
+             remember N1'eq as stayput.
+             remember N0eq as stayput1.
+           unfold updatemaps in H5.
+           simpl in H5.
+           simpl in H9.
+           apply not_true_is_false in H9.
+           rewrite H9 in H5.
+           simpl.
+           (*now have that l is not in D0*)
+           left.
+    (*inducting on T to split up W0*)
+       - inversion T; subst.
+         (*empty trace case*)
+           + 
+           inversion H; subst; try (
+                                   exfalso; by apply H5).
+           exfalso. by apply (H20 wcp).
+          (*single trace case*)
+           + destruct (iceval_cceval H H10) as [ [HN [HV Hw] ]  | [HN [HV Hw ] ] ]; subst.
+             - exfalso. by apply H5.
+             - destruct W0 as [ [W11 R1] Fw1] eqn: W1eq.
+         simpl.
+         suffices: (l \in W11).
+         intros HW1.
+         destruct (l \in Fw1) eqn: FWeq; auto.
+         apply negbT in FWeq.
+         pose proof (negfwandw_means_r TN1 FWeq HW1) as Hr.
+         simpl in Hr.
+         suffices: (
+       is_true (l \in D0)
+                   ).
+         move => contra.
++ rewrite H9 in contra. discriminate contra.
+  suffices: (is_true (l \in getdomain (NonVol M0 D0)) \/
+             is_true (l \in [::])).
+             - move => [yes | contra]. assumption.
+               rewrite in_nil in contra. discriminate contra.
+             -
+               apply (fourteen l TN1 H2); try assumption.
+               rewrite remove_empty. assumption.
+(*this comes from fact that N1 steps to M1' in one (H) but N1 l and M1' of l are different.. new theorem*)
+         assert (W11 = (getwt W0)) as Hwt. by rewrite W1eq; auto.
+         rewrite Hwt.
+         eapply wt_gets_bigger.
+         apply H.
+         (*for error 2 come here apply TN1. *)
+         rewrite <- W1eq in TN1.
+         apply TN1.
+         intros contra. subst.
+         inversion H10.
+         eapply (update_one H); try assumption.
+         intros contra. apply H5.
+         rewrite rememberme. symmetry. assumption.
+         (*big trace case*)
++ destruct W1 as [ [W11 R1] Fw1] eqn: W1eq.
+         destruct W2 as [ [W22 R2] Fw2] eqn: W2eq.
+         unfold append_write.
+         simpl.
+         suffices: (l \in Fw1).
+         intros. rewrite mem_cat.
+         apply (introT orP). by right.
+         simpl in H8.
+         suffices: (l \in W11).
+         intros HW1.
+         destruct (l \in Fw1) eqn: FWeq; auto.
+         apply negbT in FWeq.
+         pose proof (negfwandw_means_r H10 FWeq HW1) as Hr.
+         simpl in Hr.
+         suffices: (is_true (l \in Fw1 ++ remove R1 Fw2) \/
+       is_true (l \in D0)
+                   ).
+         destruct (l \in Fw1 ++ remove R1 Fw2) eqn: deq.
+         rewrite mem_cat in deq.
+         move/ orP : deq.
+         case => Hin.
+          rewrite Hin in FWeq.
+         discriminate FWeq.
+         rewrite mem_filter in Hin.
+         case/ andP : Hin => [ contra blah ].
+         rewrite Hr in contra. discriminate contra.
+         case => contra.
+         assumption.
+         rewrite H9 in contra. assumption.
+         right. rewrite rememberme1.
+         destruct3 Cmid nmid vmid cmid.
+  suffices: (is_true (l \in getdomain (NonVol M0 D0)) \/
+             is_true (l \in [::])).
+  - move => [yes | contra]. assumption.
+  rewrite in_nil in contra. discriminate contra.
+  -
+    apply (fourteen l H10 H2); try (rewrite remove_empty);
+      try assumption.
+         rewrite mem_cat in H7.
+         case/ norP : H7 => Hor1 Hor2. assumption.
+         (*this comes from fact that N1 steps to M1'
+          in one (H) but N1 l and M1' of l are different.. new theorem*)
+         assert (W11 = (getwt W1)) as Hwt. by rewrite W1eq; auto.
+         rewrite Hwt.
+         destruct3 Cmid nmid vmid cmid.
+         eapply wt_gets_bigger.
+         apply H.
+         rewrite <- W1eq in H10.
+         apply H10.
+         assumption.
+         apply (update_one H); try assumption.
+         intros contra. apply H5.
+         rewrite rememberme. symmetry. assumption.
+(*N1 l != N2 l*)
++ apply H8. by move/ eqP : beq.
+  Unshelve. apply V1. apply w. apply V1. apply w.  Qed.
+           
+
+    (*15 but multi step*)
+    Lemma twelve: forall{N0 N1 N1' N2: nvmem} {V V': vmem} {c c': command} {O: obseq} {W: the_write_stuff},
+             trace_i ((N0, V, c), N1, V, c)
+             ((N0, V, c), N1', V', c') O W ->
+             (checkpoint \notin O) ->
+             (reboot \notin O) ->
+             WARok (getdomain N0) [::] [::] c ->
+             current_init_pt N0 V c N1 N1 N2 ->
+             subset_nvm N0 N1 ->
+             current_init_pt N0 V c (N0 U! N1') (N0 U! N1') N2.
+      Admitted.
+
+(*Lemma 12.0: forall(N0 N1 N1': nvmem) (V V': vmem) (c0 c1 crem: command)
+  (Obig Osmall: obseq) (Wbig Wsmall: the_write_stuff),
+    WARok N0 [] [] [] c0 ->
+    multistep_c ((N0, V, c0), N1, V, c0) ((N0, V, c0), N1', V', c)
+    iceval ((N0, V, c0), N1, V, c0) ((N0, V, c0), N1', V', c1) Osmall Wsmall ->*)
+
+Lemma itrace_ctrace: forall{N0 N1 Nend1: nvmem} {V V' Vend: vmem} {c c' cend: command}
+                   {O : obseq} {W: the_write_stuff},
+        trace_i ((N0, V, c), N1, V', c') ((N0, V, c), Nend1, Vend, cend) O W ->
+        (reboot \notin O) ->
+        trace_c (N1, V', c') (Nend1, Vend, cend) O W.
+  Admitted.
+
+Lemma ctrace_itrace: forall(c: command) {N1 Nend1: nvmem} {V' Vend: vmem} {c' cend: command}
+                   {O : obseq} {W: the_write_stuff},
+        trace_c (N1, V', c') (Nend1, Vend, cend) O W ->
+        (forall(N0: nvmem) (V: vmem) (c: command),
+         trace_i ((N0, V, c), N1, V', c') ((N0, V, c), Nend1, Vend, cend) O W)
+        (*(reboot \notin O)*).
+  Admitted.
+(*if there is a PF it would have to be the last thing
+cuz no reboots
+ which is fine
+ cuz empty trace*)
+
+(*do implicit types for nvmem start here*)
+
+Lemma skiptrace_empty:forall{N Nend: nvmem} {V Vend: vmem} {cend: command}
+                   {O : obseq} {W: the_write_stuff},
+    trace_c (N, V, Ins skip) (Nend, Vend, cend) O W -> O = [::].
+  Admitted.
+
+Lemma ctrace_deterministic: forall{N Nend1 Nend2: nvmem} {V Vend1 Vend2: vmem} {c cend: command}
+                   {O1 O2: obseq} {W1 W2: the_write_stuff},
+        trace_c (N, V, c) (Nend1, Vend1, cend) O1 W1 ->
+        trace_c (N, V, c) (Nend2, Vend2, cend) O2 W2 ->
+        Nend1 = Nend2 /\ Vend1 = Vend2 /\ O1 = O2 /\ W1 = W2.
+  Admitted.
+
+Lemma nineteen: forall{Nstart N1 Nend N2: nvmem} {V V1 Vend: vmem} {c cend: command}
+                 {l: instruction}
+                   {O : obseq} {W: the_write_stuff},
+             same_pt Nstart V c (Ins l) N1 N2 ->
+             cceval_w (N1, V1, (Ins l)) O (Nend, Vend, cend) W ->
+            ( forall(z: loc), z \in (getrd W) -> (*z was read immediately cuz trace is only 1
+                                thing long*)
+                   (getmap N1) z = (getmap N2) z). (*since z isnt in FW of trace from Ins l to skip*)
+Admitted.
+
+Lemma twenty:
+forall{N0 N1: nvmem} {V0: vmem} {e: exp} {r0: readobs} {v0: value},
+  eeval N0 V0 e r0 v0 ->
+              (forall(z: loc), z \in (readobs_wvs r0) -> (getmap N0) z = (getmap N1) z) ->
+              eeval N1 V0 e r0 v0.
+  intros. Admitted.
+
+
+(*starting point in terms only of current mem so don't need to parameterize it,
+ don't need to induct over length of starting trace!*)
+Lemma sixteen: forall{Nstart N0 N1 Nend N2 : nvmem} {V V1 Vend: vmem}
+                {c c1 cend: command}
+                    {O Ostart: obseq} {W Wstart: the_write_stuff},
+    trace_c (Nstart, V, c) (N1, V1, c1) Ostart Wstart -> (*initializes V1 as correct*) subset_nvm N0 Nstart ->
+        trace_i ((N0, V, c), N1, V1, c1) ((N0, V, c), Nend, Vend, cend) O W -> cend <> (Ins inreboot) ->
+        (checkpoint \notin O) ->
+             (reboot \notin O) ->
+             WARok (getdomain N0) [::] [::] c ->
+             same_pt (N0 U! N1) V c c1 N1 N2 ->
+             checkpoint \notin Ostart
+           -> exists(Nend2: nvmem),(trace_c (N2, V1, c1) (Nend2, Vend, cend) O W /\
+             same_pt (N0 U! Nend) V c cend Nend Nend2).
+      intros.
+      dependent induction H1.
+      (*empty trace case*)
+      + exists N2. split. eapply CTrace_Empty.
+        assumption.
+        (*single intermittent step case*)
+      + remember H1 as Hiceval.
+        clear HeqHiceval.
+        (*show arthur the ridiculous error message
+         that i get if i take this out*)
+        (*start here consider a different
+         command type where the BC is all grouped
+         together as one instruction
+         i mean, if you wanted to do that you'd
+         induct on c
+         but i remember that being annoying for a different
+         reason
+         see how you go with this and then try it*)
+        dependent induction H1. (*induct iceval
+                                to get length of step*)
+        - (*pf*) by exfalso.
+        - (*rb*) exfalso. move/negP :H4.
+            by apply.
+        - (*cp*) exfalso. move/negP: H3. by apply.
+        - (*nv*) exists((updateNV_sv N2 x v)).
+          pose proof (NV_Assign H H0 H1) as Hcceval.
+          pose proof (iceval_cceval Hiceval Hcceval) as [ [ contraN [ contraV [contraW contrac] ] ]  | [ Hn [ Hv Hw ] ] ]; subst.
+          discriminate contrac.
+          Check nineteen.
+          pose proof (nineteen H8 Hcceval) as Hloceq.
+          Check twenty.
+          pose proof (twenty H Hloceq) as Heval2.
+          pose proof (NV_Assign Heval2 H0 H1) as Hcceval2.
+          split.
+            - by apply CTrace_Single.
+            -
+              (*showing
+  same_pt (N0 U! updateNV_sv N1 x v) V c 
+    (Ins skip) (updateNV_sv N1 x v)
+    (updateNV_sv N2 x v)
+               *)
+(*prep as i use this in multiple goals generated
+ by same_mem*)
+              assert (checkpoint \notin Ostart ++ [:: Obs r]) as Hcp.
+              apply (introT negP).
+              move => contra.
+              rewrite mem_cat in contra.
+              move/orP : contra => [contra1 | contra2].
+              apply (elimT negP) in H9.
+              (*ask arthur how is it that those switch*)
+                by apply H9.
+                rewrite mem_seq1 in contra2.
+                  by move/eqP : contra2.
+              inversion H8. subst.
+              eapply same_mem; try auto.
+              (*consider is there any point to the
+               multistep part*)
+            - (*showing
+  trace_c (N0 U! updateNV_sv N1 x v, V, c)
+    (updateNV_sv N1 x v, ?V1, Ins skip) 
+    ?O1 ?W1
+               *)
+              (*NTS crem = skip*)
+              pose proof (trace_stops T2) as Hrem.
+              pose proof (trace_append T1 T2) as Tend.
+              pose proof (and_or_elim Hrem H10).
+              assert (~
+        (crem = Ins (asgn_sv x e) /\
+         (exists w crem2, crem = incheckpoint w;; crem2))).
+              intros [contra1 [b1 [b2 contra2] ] ].
+              subst. discriminate contra2.
+              apply H15 in H16. subst.
+              (*make Hcceval into a continuous trace,
+               combine it with H2*)
+pose proof (trace_append H2 (CTrace_Single Hcceval)) as Tcs2e.
+                assert (multi_step_i (N0, V, c, Nstart,
+                                     V, c)
+                                     (N0, V, c, (updateNV_sv N1 x v), Vend, Ins skip) (Ostart ++ [:: Obs r])) as Ts2e.
+pose proof (ctrace_itrace c Tcs2e).
+exists (append_write Wstart
+             ([:: inl x],
+             readobs_wvs r,
+             remove
+               (readobs_wvs r)
+               [:: inl x])).
+eapply H16.
+              pose proof (
+                     twelve00 Ts2e Hcp H7 H3 Tcs2e Hcp
+                   ) as Tends2end.
+              apply Tends2end.
+        - (*showing
+  trace_c (updateNV_sv N1 x v, Vend, Ins skip)
+(?N2, ?V2, ?crem) ?O2 ?W2 *)
+          apply CTrace_Empty. apply Hcp.
+          auto.
+          simpl.
+     (*showing N1 =1 N2*)
+      - intros l contra.
+              (*start here you'd think there'd be some
+               sort of reboots req for first trace in twelve00*)
+              
+              Admitted.
+           (*     pose proof (twelve00 Hm H3 H5
+                           )
+              apply (iTrace_Single Hiceval) .
+(*ask arthur can i use exist in a function
+ sort of way*)
+              suffices: (trace_c updateNV_sv N1 x v, V, c)
+              pose proof (single_step_all
+                         (CTrace_Single Hcceval))
+        (*kind of weird that the restarting actually takes
+         2 steps with this RB step in the middle,
+         maybe easier if we handled restarting in the base case?*)
+        (*induct on instruction to get correct map*)
+        induction l.
+      - (*skip*) inversion H; subst. by exfalso.
+      -
+        exists((updateNV_sv N2 x v))
+        (*apply 19*)*)
+
+
+      (*ask arthur i want this enforced at the type level*)
+    Lemma dom_eq: forall(N0 N1: nvmem),
+        (getmap N0) =1 (getmap N1) ->
+        N0 = N1.
+      Admitted.
+
+Lemma eleven_bc: forall{N0 N1 Nmid Nend N2: nvmem} {V Vmid Vend: vmem} {c cmid cend: command}
+                  {O1 Orem: obseq} {W1 Wrem: the_write_stuff},
+        (*need the N0 here cuz of same config*)
+        trace_i ((N0, V, c), N1, V, c) ((N0, V, c), Nmid, Vmid, cmid) O1 W1 ->
+        (checkpoint \notin O1) ->
+        (reboot \notin O1) ->
+             subset_nvm N0 N1 ->
+             subset_nvm N0 N2 ->
+             current_init_pt N0 V c N1 N1 N2 ->
+             WARok (getdomain N0) [::] [::] c ->
+             trace_i ((N0, V, c), Nmid, Vmid, cmid) ((N0, V, c), Nend, Vend, cend) Orem Wrem ->
+             (* Sigma -> Sigma'
+configs can always make progress assumption*)
+             (checkpoint \notin Orem) ->
+             (reboot \notin Orem) ->
+             ((cend = Ins skip) \/ exists(w: warvars) (cend2: command), cend = (incheckpoint w);; cend2) ->
+             (exists(sigma: context) (Wc:
+                                            the_write_stuff),
+                 trace_c (N2, V, c) sigma O1 Wc /\
+                         (*write SETS have to be the same
+                          but write lists do not,
+                          can add that extra specificity
+                          if I need it*)
+             same_config ((N0, V, c), Nmid, Vmid, cmid) (*Sigma ~ sigma*)
+                         sigma /\
+             trace_c sigma (Nend, Vend, cend) Orem Wrem (*sigma -> Sigma'-*)
+             (*same obs, write as "intermittent" execution*)
+             ).
+  intros.
+        suffices: exists(Nmid2: nvmem),
+          (trace_c (N2, V, c) (Nmid2, Vmid, cmid) O1 W1 /\
+           same_pt (N0 U! Nmid) V c cmid Nmid Nmid2).
+      - move => [Nmid2 [Tc1 Hsp] ].
+        exists (Nmid2, Vmid, cmid) W1. split.
+        + assumption.
+        + split.
+           - constructor. assumption.
+           - (*trying to use 16 instead of 17*)
+            (* destruct H8 as [H80 | H81].*)
+           (*  subst.
+             split.
+             +*)
+               assert (cend <> (Ins inreboot)) as Hcend.
+               - intros contra. subst.
+                 destruct H9 as [contra1 | [b1 [b2 contra2] ] ].
+                 discriminate contra1.
+                 discriminate contra2.
+                 Check sixteen.
+               destruct (sixteen H6 Hcend H7 H8 H5 Hsp)
+                 as [Nend2 [Tc2 Hspend] ].
+               suffices: Nend = Nend2.
+               move=> Heq. subst. assumption.
+           - inversion Hspend. subst.
+             apply dom_eq.
+             intros l.
+             apply: eqP.
+             apply: negPn.
+             (*start here why didn't normal apply work*)
+             apply (introT negP).
+             move/ eqP => contra.
+             apply H14 in contra.
+             destruct contra as [contra0 [contra1 contra2] ].
+             (*now showing that W2 is empty*)
+               destruct H9 as [H81 | H82]; subst.
+             pose proof (skiptrace_empty T2). subst.
+             apply empty_trace in T2; auto. destruct T2 as [Heq1 Heq2]. subst.
+             rewrite in_nil in contra0. discriminate contra0.
+             destruct H82 as [w [cend2 Heqcend] ]. subst.
+             pose proof (observe_checkpt T2) as
+                 [contra3 | contra3].
+             subst.
+             apply empty_trace_sc in T2.
+             destruct T2 as [blah [blah1 [blah2 blah3] ] ].
+             subst.
+             rewrite in_nil in contra0. discriminate contra0.
+               by apply: (negP H13).
+   - eapply sixteen; try eapply iTrace_Empty; try
+        (*how is auto too stupid to solve this*)
+                                                (by rewrite in_nil); try assumption. apply H. intros contra. subst.
+     pose proof (observe_rb H6) as contra.
+     destruct contra as [contra1 | contra2]; subst.
+     destruct H9 as [contra1 | [b1 [b2 contra2] ] ].
+     discriminate contra1. discriminate contra2.
+     move/negP : H8.
+     by apply.
+     (* start here
+pretty cool that this works given the theorem statement of
+update_sub rewrite - {1} (update_sub H1).*)
+     rewrite {1} (update_sub H2).
+     eapply eight; try apply H2; try assumption.
+     Qed.
+
+      Lemma obseq_readobs: forall{O: obseq}
+                            {N1 N2: nvmem}
+                            {V1 V2: vmem}
+                            {c1 c2: command}
+                            {W: the_write_stuff},
+trace_c (N1, V1, c1) (N2, V2, c2) O
+        W ->
+checkpoint \notin O ->
+exists(o: readobs), O = [::Obs o].
+Admitted.
+
+Lemma hacky: forall(o3 o4: readobs),
+                    [:: Obs o3] ++ [:: Obs o4] =
+              [:: Obs (o3 ++ o4)].
+Admitted.
+
+      Lemma can_make_progress: forall(N: nvmem) (V: vmem)
+                                (c: command),
+                                  exists(Nend: nvmem) (Vend: vmem)
+                                   (cend: command)
+                                   (O: obseq)
+                                  (W: the_write_stuff),
+                                    trace_c (N, V, c) (Nend, Vend, cend) O W /\ checkpoint \notin O /\
+(cend = Ins skip \/
+        (exists w cend2,
+            cend = incheckpoint w;; cend2)).
+        Admitted.
+
+Lemma same_nearest_CP: forall{Ns Nend1 Nend2: nvmem} {Vs Vend1
+                                            Vend2: vmem}
+                {c cend1 cend2: command} {O1 O2: obseq}
+                {W1 W2: the_write_stuff},
+    trace_c (Ns, Vs, c) (Nend1, Vend1, cend1) O1 W1 ->
+    checkpoint \notin O1 ->
+    (cend1 = Ins skip \/
+     (exists w1 crem1, cend1 = incheckpoint w1;; crem1))
+      (*start here make that into a prop*) ->
+    trace_c (Ns, Vs, c) (Nend2, Vend2, cend2) O2 W2 ->
+    checkpoint \notin O2 -> 
+    (cend2 = Ins skip \/
+     (exists w2 crem2, cend2 = incheckpoint w2;; crem2))
+   -> cend1 = cend2.
+Admitted.
+
+    Lemma eleven: forall{N0 N1 Nmid Nend N2: nvmem} {V Vmid Vend: vmem} {c cmid cend: command}
+                   {O1 Orem: obseq} {W1 Wrem: the_write_stuff},
+        trace_i ((N0, V, c), N1, V, c) ((N0, V, c), Nmid, Vmid, cmid) O1 W1 ->
+             (checkpoint \notin O1) ->
+             subset_nvm N0 N1 ->
+             subset_nvm N0 N2 ->
+             current_init_pt N0 V c N1 N1 N2 ->
+             WARok (getdomain N0) [::] [::] c ->
+             trace_i ((N0, V, c), Nmid, Vmid, cmid) ((N0, V, c), Nend, Vend, cend) Orem Wrem ->
+             (* Sigma -> Sigma'
+configs can always make progress assumption*)
+             (checkpoint \notin Orem) ->
+             (reboot \notin Orem) ->
+             ((cend = Ins skip) \/ exists(w: warvars) (cend2: command), cend = (incheckpoint w);; cend2) ->
+             (exists(O2: obseq) (sigma: context) (Wc:
+                                            the_write_stuff),
+                 trace_c (N2, V, c) sigma O2 Wc /\
+                 checkpoint \notin O2 /\ (*cuz its taking
+                                         the same path as N1 to
+                                         cmid*)
+                 (*write SETS have to be the same
+                          but write lists do not,
+                          can add that extra specificity
+                          if I need it*)
+             same_config ((N0, V, c), Nmid, Vmid, cmid) (*Sigma ~ sigma*)
+                         sigma /\
+             trace_c sigma (Nend, Vend, cend) Orem Wrem  /\ (*sigma -> Sigma'-*)
+             (*same obs, write as "intermittent" execution*)
+             (O1 ++ Orem <=m O2 ++ Orem)).
+      intros.
+      apply trace_convert in H.
+      dependent induction H.
+      2: {
+        suffices: (exists O3 sigma Wc,
+               trace_c (N2, V, c) sigma O3 Wc /\
+                      is_true (checkpoint \notin O3) /\
+               same_config
+                 (N0, V, c, Nmid, Vmid, cmid)
+                 sigma /\
+               trace_c sigma (Nend, Vend, cend)
+                 Orem Wrem /\
+               (O2 ++ Orem <=m O3 ++ Orem)).
+      - intros [O3 [sigma [Wc [Hc1 [Hc2 [Hc3 [ Hc4 Hc5 ]
+                   ] ] ] ] ] ].
+      exists O3, sigma, Wc.
+      repeat (try split); try assumption.
+      destruct3 sigma Ns Vs cs.
+      pose proof (obseq_readobs Hc1 Hc2) as [o3 Ho3].
+      pose proof (obseq_readobs Hc4 H9) as [o4 Ho4].
+      pose proof (obseq_readobs H H1) as [o1 Ho1].
+      (*dont think obseq_readobs is actually true
+       because the trace doesnt append consecutive read observations together*
+      why do i even need the above
+       to get it to match the structure of RB_IND w a singleton on the
+       right. if i didnt bunch readobs up into one list, wouldnt need*)
+      subst.
+      repeat rewrite - catA.
+      rewrite~ (hacky o3 o4).
+      apply RB_Ind.
+      (*2nd goal should come out of Hc5*)
+      Check eleven_bc.
+      assert (reboot \notin [:: Obs o1]) as Ho1.
+      apply (introT negP).
+      rewrite mem_seq1. move/eqP => contra. discriminate contra.
+      pose proof (can_make_progress Nmid0 Vmid0 cmid0) as
+          [Nend1 [Vend1 [cend1 [Oend1 [Wend1 [Tendc [Hcend1
+                 Hcend2]  ] ] ] ] ] ].
+      pose proof (obseq_readobs Tendc Hcend1) as [oend Hoend].
+      subst.
+      assert (reboot \notin [:: Obs oend]) as Hoend.
+      apply (introT negP).
+      rewrite mem_seq1. move/eqP => contra. discriminate contra.
+      Check eleven_bc.
+      rewrite mem_cat negb_orb in H3.
+      move/ andP : H3 => [H31 H32].
+      Check eleven_bc.
+      pose proof (iTrace_Cont N0 V c H H31) as Hi.
+      pose proof (iTrace_Cont N0 V c Tendc Hcend1) as Tendci.
+      (*consider having two directions for trace_Convertso that
+       you can combine this*)
+      apply trace_convert in Hi. apply trace_convert in Tendci.
+      pose proof (eleven_bc Hi H31 Ho1 H4 H5 H6 H7
+                           Tendci 
+                            Hcend1 Hoend
+                            Hcend2)
+      as [ [ [Ns1 Vs1] cs1]  [Wc1 [Hc11 [Hc21 Hc31]
+         ] ] ].
+      pose proof (trace_append Hc11 Hc31) as Hc2end1.
+      pose proof (trace_append Hc1 Hc4) as Hc2end.
+      assert (checkpoint \notin [:: Obs o3] ++ [:: Obs o4])
+        as Hcp1.
+      apply (introT negP). intros contra.
+      rewrite mem_cat in contra.
+      move/orP : contra => [contra1 | contra2].
+      move/negP : Hc2. by apply.
+      move/negP : H9. by apply.
+      assert (checkpoint \notin ([:: Obs o1] ++ [:: Obs oend]))
+        as Hcp2.
+      apply (introT negP). intros contra.
+      rewrite mem_cat in contra.
+      move/orP : contra => [contra1 | contra2].
+      move/negP : H31. by apply.
+      move/negP : Hcend1. by apply.
+      pose proof (same_nearest_CP Hc2end Hcp1 H11 Hc2end1 Hcp2 Hcend2). subst.
+      apply (ctrace_deterministic Hc2end1) in Hc2end.
+      destruct Hc2end as [e1 [e2 [e3 e4] ] ]. subst.
+      exists (size o1).
+      repeat rewrite hacky in e3.
+      inversion e3. subst.
+        by rewrite take_size_cat.
+          by rewrite hacky in Hc5.
+      - eapply IHtrace_i1; try reflexivity; try assumption.
+        apply sub_update.
+        Check twelve.
+        (*might make my life easier to have 12 take in a continuous trace*)
+        pose proof (iTrace_Cont N0 V c H H1) as T12.
+        apply trace_convert in T12.
+        eapply (twelve T12 H1
+                       (neg_observe_rb H)
+                       H7 H6 H4).
+        (*i think this is 12*)
+(* ask arthur am i stupid or this should do something
+ unfold prefix in Hc51*)
+
+      (*split up Hc2end
+Hc51 should give it
+       *)
+
+
+
+     (* ask arthur.. seriously?
+pose proof (and4 Hc1 Hc2 Hc3 Hc4) as Hc.
+Record types where each one of those guys is a field
+      *)
+
+
+
+
+
+ (*   Lemma eleven1: forall{N0 N1 Nmid Nend N2: nvmem} {V Vmid Vend: vmem} {c cmid cend: command}
+                   {O1 Orem: obseq} {W1 Wrem: the_write_stuff},
+        trace_i ((N0, V, c), N1, V, c) ((N0, V, c), Nmid, Vmid, cmid) O1 W1 ->
+             (checkpoint \notin O1) ->
+             subset_nvm N0 N1 ->
+             subset_nvm N0 N2 ->
+             current_init_pt N0 V c N1 N1 N2 ->
+             WARok (getdomain N0) [::] [::] c ->
+             trace_i ((N0, V, c), Nmid, Vmid, cmid) ((N0, V, c), Nend, Vend, cend) Orem Wrem ->
+             (* Sigma -> Sigma'
+configs can always make progress assumption*)
+             (checkpoint \notin Orem) ->
+             (reboot \notin Orem) ->
+             ((cend = Ins skip) \/ exists(w: warvars) (cend2: command), cend = (incheckpoint w);; cend2) ->
+             (exists(O2: obseq) (sigma: context) (Wc:
+                                            the_write_stuff),
+                 trace_c (N2, V, c) sigma O2 Wc /\
+                         (*write SETS have to be the same
+                          but write lists do not,
+                          can add that extra specificity
+                          if I need it*)
+             same_config ((N0, V, c), Nmid, Vmid, cmid) (*Sigma ~ sigma*)
+                         sigma /\
+             trace_c sigma (Nend, Vend, cend) Orem Wrem  /\ (*sigma -> Sigma'-*)
+             (*same obs, write as "intermittent" execution*)
+             O1 ++ Orem <= O2 ++ Orem).
+      intros.
+      (*inducting on reboots in start => Sigma*)
+      + dependent induction H using reboot_ind.
+        (*ask arthur bad induction principl here ):*)
+        destruct ((count_reboots H) == O) eqn: BC.
+        move/ eqP / count_memPn : BC => BC.
+        (*base case*)
+      +
+        suffices: exists(Nmid2: nvmem),
+          (trace_c (N2, V, c) (Nmid2, Vmid, cmid) O1 W1 /\
+           same_pt (N0 U! Nmid) V c cmid Nmid Nmid2).
+      - move => [Nmid2 [Tc1 Hsp] ].
+        exists O1 (Nmid2, Vmid, cmid) W1. split.
+        + assumption.
+        + split.
+           - constructor. assumption.
+           - (*trying to use 16 instead of 17*)
+            (* destruct H8 as [H80 | H81].*)
+             subst.
+             split.
+             +
+               assert (cend <> (Ins inreboot)) as Hcend.
+               - intros contra. subst.
+                 destruct H8 as [contra1 | [b1 [b2 contra2] ] ].
+                 discriminate contra1.
+                 discriminate contra2.
+                 Check sixteen.
+               destruct (sixteen H5 Hcend H6 H7 H4 Hsp)
+                 as [Nend2 [Tc2 Hspend] ].
+               suffices: Nend = Nend2.
+               move=> Heq. subst. assumption.
+           - inversion Hspend. subst.
+             apply dom_eq.
+             intros l.
+             apply: eqP.
+             apply: negPn.
+             (*start here why didn't normal apply work*)
+             apply (introT negP).
+             move/ eqP => contra.
+             apply H14 in contra.
+             destruct contra as [contra0 [contra1 contra2] ].
+             (*now showing that W2 is empty*)
+               destruct H8 as [H81 | H82]; subst.
+             pose proof (skiptrace_empty T2). subst.
+             apply empty_trace in T2; auto. destruct T2 as [Heq1 Heq2]. subst.
+             (*ask arthur how the above works with applying it
+              for you sort of*)
+             rewrite in_nil in contra0. discriminate contra0.
+             destruct H82 as [w [cend2 Heqcend] ]. subst.
+             pose proof (observe_checkpt T2) as
+                 [contra3 | contra3].
+             subst.
+             apply empty_trace_sc in T2.
+             destruct T2 as [blah [blah1 [blah2 blah3] ] ].
+             subst.
+             rewrite in_nil in contra0. discriminate contra0.
+               by apply: (negP H13).
+      + exists (size (O1 ++ Orem)). rewrite* take_size.
+   - eapply sixteen; try eapply iTrace_Empty; try
+        (*how is auto too stupid to solve this*)
+                                                (by rewrite in_nil); try assumption. apply H. intros contra. subst.
+     pose proof (observe_rb H5) as contra.
+     destruct contra as [contra1 | contra2]; subst.
+     destruct H8 as [contra1 | [b1 [b2 contra2] ] ].
+     discriminate contra1. discriminate contra2.
+     move/negP : H7.
+     by apply.
+     (* start here
+pretty cool that this works given the theorem statement of
+update_sub rewrite - {1} (update_sub H1).*)
+     rewrite {1} (update_sub H1).
+     eapply eight; try apply H1; try assumption.
+(*IH is NOT general enough*)
+     Lemma split_rb: forall{N0, N1, Nend: nvmem}
+                      {V}
+
+     (*base case done!*)
+
+     
+        
+             destruct H10 as [H100 | H101].
+           - (*both skip case*)
+             pose proof (skiptrace_empty T2). subst.
+             destruct (empty_trace T2); auto. subst.
+
+             destruct H82 as [w [cend2 Hcendeq] ].
+             subst.
+             pose proof (observe_checkpt T2) as
+                 [contra3 | contra3].
+             discriminate contra3.
+             move/ negP : H13. by apply.
+             pose proof (skiptrace_empty T2). subst.
+             apply empty_trace in T2. destruct T2 as [Heq1 Heq2].
+             subst. rewrite in+nil in contra
+               in_nil in contra0.
+             discriminate contra0.
+             inversion H8.
+
+             apply: negP.
+             apply negbT.
+             apply: negP.
+             (*should be a way to combine those two start here*)
+              introT negPn (elimT eqP)
+             extensionality.
+ose proof (eight H1 H2 H3) as Height.
+               Check sixteen.
+               inversion Hsp. subst.
+               Check itrace_ctrace.
+               pose proof (itrace_ctrace H5 H7) as Tc3.
+               destruct (ctrace_deterministic )
+               ctrace_det
+               (*worry about H11 in a second*)
+               suffices: Nend = Nend2.
+               move => Heq. subst. assumption.
+               inversion Hspend. subst.
+               destruct H8 as [H81 | H82].
+               destruct H10 as [H101 | H102].
+               subst.
+(*wiggle with samept and the fact that cend
+ is \/ by H8*)
+
+
+                     iceval_w ((N0, V, c), N1, V, c) O
+             ((N0, V, c), N1', V', c') W ->
+             (reboot \notin O) ->
+             WARok (getdomain N0) [::] [::] c ->
+             current_init_pt N0 V c N1 N1 N2 ->
+             current_init_pt N0 V c (N0 U! N1') (N0 U! N1')*)
